---
layout: default
title : "Base.Homomorphisms.Products module (The Agda Universal Algebra Library)"
date : "2021-09-08"
author: "agda-algebras development team"
---

### <a id="products-of-homomorphisms">Products of Homomorphisms</a>

This is the [Base.Homomorphisms.Products] module of the [Agda Universal Algebra Library][].

<pre class="Agda">

<a id="345" class="Symbol">{-#</a> <a id="349" class="Keyword">OPTIONS</a> <a id="357" class="Pragma">--without-K</a> <a id="369" class="Pragma">--exact-split</a> <a id="383" class="Pragma">--safe</a> <a id="390" class="Symbol">#-}</a>

<a id="395" class="Keyword">open</a> <a id="400" class="Keyword">import</a> <a id="407" href="Overture.html" class="Module">Overture</a> <a id="416" class="Keyword">using</a> <a id="422" class="Symbol">(</a><a id="423" href="Overture.Signatures.html#3264" class="Function">Signature</a> <a id="433" class="Symbol">;</a> <a id="435" href="Overture.Signatures.html#648" class="Generalizable">𝓞</a> <a id="437" class="Symbol">;</a> <a id="439" href="Overture.Signatures.html#650" class="Generalizable">𝓥</a> <a id="441" class="Symbol">)</a>

<a id="444" class="Keyword">module</a> <a id="451" href="Base.Homomorphisms.Products.html" class="Module">Base.Homomorphisms.Products</a> <a id="479" class="Symbol">{</a><a id="480" href="Base.Homomorphisms.Products.html#480" class="Bound">𝑆</a> <a id="482" class="Symbol">:</a> <a id="484" href="Overture.Signatures.html#3264" class="Function">Signature</a> <a id="494" href="Overture.Signatures.html#648" class="Generalizable">𝓞</a> <a id="496" href="Overture.Signatures.html#650" class="Generalizable">𝓥</a><a id="497" class="Symbol">}</a> <a id="499" class="Keyword">where</a>

<a id="506" class="Comment">-- Imports from Agda and the Agda Standard Library -----------------------</a>
<a id="581" class="Keyword">open</a> <a id="586" class="Keyword">import</a> <a id="593" href="Agda.Primitive.html" class="Module">Agda.Primitive</a>  <a id="609" class="Keyword">using</a> <a id="615" class="Symbol">()</a> <a id="618" class="Keyword">renaming</a> <a id="627" class="Symbol">(</a> <a id="629" href="Agda.Primitive.html#388" class="Primitive">Set</a> <a id="633" class="Symbol">to</a> <a id="636" class="Primitive">Type</a> <a id="641" class="Symbol">)</a>
<a id="643" class="Keyword">open</a> <a id="648" class="Keyword">import</a> <a id="655" href="Data.Product.html" class="Module">Data.Product</a>    <a id="671" class="Keyword">using</a> <a id="677" class="Symbol">(</a> <a id="679" href="Agda.Builtin.Sigma.html#235" class="InductiveConstructor Operator">_,_</a> <a id="683" class="Symbol">)</a>
<a id="685" class="Keyword">open</a> <a id="690" class="Keyword">import</a> <a id="697" href="Level.html" class="Module">Level</a>           <a id="713" class="Keyword">using</a> <a id="719" class="Symbol">(</a> <a id="721" href="Agda.Primitive.html#742" class="Postulate">Level</a> <a id="727" class="Symbol">;</a>  <a id="730" href="Agda.Primitive.html#961" class="Primitive Operator">_⊔_</a> <a id="734" class="Symbol">;</a> <a id="736" href="Agda.Primitive.html#931" class="Primitive">suc</a> <a id="740" class="Symbol">)</a>

<a id="743" class="Keyword">open</a> <a id="748" class="Keyword">import</a> <a id="755" href="Relation.Binary.PropositionalEquality.html" class="Module">Relation.Binary.PropositionalEquality</a> <a id="793" class="Keyword">using</a> <a id="799" class="Symbol">(</a> <a id="801" href="Agda.Builtin.Equality.html#207" class="InductiveConstructor">refl</a> <a id="806" class="Symbol">)</a>

<a id="809" class="Keyword">open</a> <a id="814" class="Keyword">import</a> <a id="821" href="Axiom.Extensionality.Propositional.html" class="Module">Axiom.Extensionality.Propositional</a> <a id="856" class="Keyword">renaming</a> <a id="865" class="Symbol">(</a><a id="866" href="Axiom.Extensionality.Propositional.html#750" class="Function">Extensionality</a> <a id="881" class="Symbol">to</a> <a id="884" class="Function">funext</a><a id="890" class="Symbol">)</a>
  <a id="894" class="Keyword">using</a> <a id="900" class="Symbol">()</a>

<a id="904" class="Comment">-- Imports from the Agda Universal Algebras Library ----------------------</a>
<a id="979" class="Keyword">open</a> <a id="984" class="Keyword">import</a> <a id="991" href="Overture.html" class="Module">Overture</a> <a id="1000" class="Keyword">using</a> <a id="1006" class="Symbol">(</a> <a id="1008" href="Overture.Basic.html#4325" class="Function Operator">∣_∣</a> <a id="1012" class="Symbol">;</a> <a id="1014" href="Overture.Basic.html#4363" class="Function Operator">∥_∥</a><a id="1017" class="Symbol">)</a>

<a id="1020" class="Keyword">open</a> <a id="1025" class="Keyword">import</a> <a id="1032" href="Base.Algebras.html" class="Module">Base.Algebras</a>             <a id="1058" class="Symbol">{</a><a id="1059" class="Argument">𝑆</a> <a id="1061" class="Symbol">=</a> <a id="1063" href="Base.Homomorphisms.Products.html#480" class="Bound">𝑆</a><a id="1064" class="Symbol">}</a>  <a id="1067" class="Keyword">using</a> <a id="1073" class="Symbol">(</a> <a id="1075" href="Base.Algebras.Basic.html#2774" class="Function">Algebra</a> <a id="1083" class="Symbol">;</a> <a id="1085" href="Base.Algebras.Products.html#1923" class="Function">⨅</a> <a id="1087" class="Symbol">)</a>
<a id="1089" class="Keyword">open</a> <a id="1094" class="Keyword">import</a> <a id="1101" href="Base.Homomorphisms.Basic.html" class="Module">Base.Homomorphisms.Basic</a>  <a id="1127" class="Symbol">{</a><a id="1128" class="Argument">𝑆</a> <a id="1130" class="Symbol">=</a> <a id="1132" href="Base.Homomorphisms.Products.html#480" class="Bound">𝑆</a><a id="1133" class="Symbol">}</a>  <a id="1136" class="Keyword">using</a> <a id="1142" class="Symbol">(</a> <a id="1144" href="Base.Homomorphisms.Basic.html#2734" class="Function">hom</a> <a id="1148" class="Symbol">;</a> <a id="1150" href="Base.Homomorphisms.Basic.html#4290" class="Function">epi</a> <a id="1154" class="Symbol">)</a>

<a id="1157" class="Keyword">private</a> <a id="1165" class="Keyword">variable</a> <a id="1174" href="Base.Homomorphisms.Products.html#1174" class="Generalizable">𝓘</a> <a id="1176" href="Base.Homomorphisms.Products.html#1176" class="Generalizable">β</a> <a id="1178" class="Symbol">:</a> <a id="1180" href="Agda.Primitive.html#742" class="Postulate">Level</a>

</pre>

Suppose we have an algebra `𝑨`, a type `I : Type 𝓘`, and a family `ℬ : I → Algebra β` of algebras.  We sometimes refer to the inhabitants of `I` as *indices*, and call `ℬ` an *indexed family of algebras*.

If in addition we have a family `𝒽 : (i : I) → hom 𝑨 (ℬ i)` of homomorphisms, then we can construct a homomorphism from `𝑨` to the product `⨅ ℬ` in the natural way.

<pre class="Agda">

<a id="1585" class="Keyword">module</a> <a id="1592" href="Base.Homomorphisms.Products.html#1592" class="Module">_</a> <a id="1594" class="Symbol">{</a><a id="1595" href="Base.Homomorphisms.Products.html#1595" class="Bound">I</a> <a id="1597" class="Symbol">:</a> <a id="1599" href="Base.Homomorphisms.Products.html#636" class="Primitive">Type</a> <a id="1604" href="Base.Homomorphisms.Products.html#1174" class="Generalizable">𝓘</a><a id="1605" class="Symbol">}(</a><a id="1607" href="Base.Homomorphisms.Products.html#1607" class="Bound">ℬ</a> <a id="1609" class="Symbol">:</a> <a id="1611" href="Base.Homomorphisms.Products.html#1595" class="Bound">I</a> <a id="1613" class="Symbol">→</a> <a id="1615" href="Base.Algebras.Basic.html#2774" class="Function">Algebra</a> <a id="1623" href="Base.Homomorphisms.Products.html#1176" class="Generalizable">β</a><a id="1624" class="Symbol">)</a> <a id="1626" class="Keyword">where</a>

 <a id="1634" href="Base.Homomorphisms.Products.html#1634" class="Function">⨅-hom-co</a> <a id="1643" class="Symbol">:</a>  <a id="1646" href="Base.Homomorphisms.Products.html#884" class="Function">funext</a> <a id="1653" href="Base.Homomorphisms.Products.html#1604" class="Bound">𝓘</a> <a id="1655" href="Base.Homomorphisms.Products.html#1623" class="Bound">β</a> <a id="1657" class="Symbol">→</a> <a id="1659" class="Symbol">{</a><a id="1660" href="Base.Homomorphisms.Products.html#1660" class="Bound">α</a> <a id="1662" class="Symbol">:</a> <a id="1664" href="Agda.Primitive.html#742" class="Postulate">Level</a><a id="1669" class="Symbol">}(</a><a id="1671" href="Base.Homomorphisms.Products.html#1671" class="Bound">𝑨</a> <a id="1673" class="Symbol">:</a> <a id="1675" href="Base.Algebras.Basic.html#2774" class="Function">Algebra</a> <a id="1683" href="Base.Homomorphisms.Products.html#1660" class="Bound">α</a><a id="1684" class="Symbol">)</a>
  <a id="1688" class="Symbol">→</a>           <a id="1700" class="Symbol">(∀(</a><a id="1703" href="Base.Homomorphisms.Products.html#1703" class="Bound">i</a> <a id="1705" class="Symbol">:</a> <a id="1707" href="Base.Homomorphisms.Products.html#1595" class="Bound">I</a><a id="1708" class="Symbol">)</a> <a id="1710" class="Symbol">→</a> <a id="1712" href="Base.Homomorphisms.Basic.html#2734" class="Function">hom</a> <a id="1716" href="Base.Homomorphisms.Products.html#1671" class="Bound">𝑨</a> <a id="1718" class="Symbol">(</a><a id="1719" href="Base.Homomorphisms.Products.html#1607" class="Bound">ℬ</a> <a id="1721" href="Base.Homomorphisms.Products.html#1703" class="Bound">i</a><a id="1722" class="Symbol">))</a> <a id="1725" class="Symbol">→</a> <a id="1727" href="Base.Homomorphisms.Basic.html#2734" class="Function">hom</a> <a id="1731" href="Base.Homomorphisms.Products.html#1671" class="Bound">𝑨</a> <a id="1733" class="Symbol">(</a><a id="1734" href="Base.Algebras.Products.html#1923" class="Function">⨅</a> <a id="1736" href="Base.Homomorphisms.Products.html#1607" class="Bound">ℬ</a><a id="1737" class="Symbol">)</a>

 <a id="1741" href="Base.Homomorphisms.Products.html#1634" class="Function">⨅-hom-co</a> <a id="1750" href="Base.Homomorphisms.Products.html#1750" class="Bound">fe</a> <a id="1753" href="Base.Homomorphisms.Products.html#1753" class="Bound">𝑨</a> <a id="1755" href="Base.Homomorphisms.Products.html#1755" class="Bound">𝒽</a> <a id="1757" class="Symbol">=</a> <a id="1759" class="Symbol">(λ</a> <a id="1762" href="Base.Homomorphisms.Products.html#1762" class="Bound">a</a> <a id="1764" href="Base.Homomorphisms.Products.html#1764" class="Bound">i</a> <a id="1766" class="Symbol">→</a> <a id="1768" href="Overture.Basic.html#4325" class="Function Operator">∣</a> <a id="1770" href="Base.Homomorphisms.Products.html#1755" class="Bound">𝒽</a> <a id="1772" href="Base.Homomorphisms.Products.html#1764" class="Bound">i</a> <a id="1774" href="Overture.Basic.html#4325" class="Function Operator">∣</a> <a id="1776" href="Base.Homomorphisms.Products.html#1762" class="Bound">a</a><a id="1777" class="Symbol">)</a> <a id="1779" href="Agda.Builtin.Sigma.html#235" class="InductiveConstructor Operator">,</a> <a id="1781" class="Symbol">λ</a> <a id="1783" href="Base.Homomorphisms.Products.html#1783" class="Bound">𝑓</a> <a id="1785" href="Base.Homomorphisms.Products.html#1785" class="Bound">𝒶</a> <a id="1787" class="Symbol">→</a> <a id="1789" href="Base.Homomorphisms.Products.html#1750" class="Bound">fe</a> <a id="1792" class="Symbol">λ</a> <a id="1794" href="Base.Homomorphisms.Products.html#1794" class="Bound">i</a> <a id="1796" class="Symbol">→</a> <a id="1798" href="Overture.Basic.html#4363" class="Function Operator">∥</a> <a id="1800" href="Base.Homomorphisms.Products.html#1755" class="Bound">𝒽</a> <a id="1802" href="Base.Homomorphisms.Products.html#1794" class="Bound">i</a> <a id="1804" href="Overture.Basic.html#4363" class="Function Operator">∥</a> <a id="1806" href="Base.Homomorphisms.Products.html#1783" class="Bound">𝑓</a> <a id="1808" href="Base.Homomorphisms.Products.html#1785" class="Bound">𝒶</a>

</pre>

The foregoing generalizes easily to the case in which the domain is also a product
of a family of algebras. That is, if we are given `𝒜 : I → Algebra α` and
`ℬ : I → Algebra β` (two families of `𝑆`-algebras), and
`𝒽 :  Π i ꞉ I , hom (𝒜 i)(ℬ i)` (a family of homomorphisms), then we can
construct a homomorphism from `⨅ 𝒜` to `⨅ ℬ` in the following natural way.

<pre class="Agda">

 <a id="2200" href="Base.Homomorphisms.Products.html#2200" class="Function">⨅-hom</a> <a id="2206" class="Symbol">:</a>  <a id="2209" href="Base.Homomorphisms.Products.html#884" class="Function">funext</a> <a id="2216" href="Base.Homomorphisms.Products.html#1604" class="Bound">𝓘</a> <a id="2218" href="Base.Homomorphisms.Products.html#1623" class="Bound">β</a> <a id="2220" class="Symbol">→</a> <a id="2222" class="Symbol">{</a><a id="2223" href="Base.Homomorphisms.Products.html#2223" class="Bound">α</a> <a id="2225" class="Symbol">:</a> <a id="2227" href="Agda.Primitive.html#742" class="Postulate">Level</a><a id="2232" class="Symbol">}(</a><a id="2234" href="Base.Homomorphisms.Products.html#2234" class="Bound">𝒜</a> <a id="2236" class="Symbol">:</a> <a id="2238" href="Base.Homomorphisms.Products.html#1595" class="Bound">I</a> <a id="2240" class="Symbol">→</a> <a id="2242" href="Base.Algebras.Basic.html#2774" class="Function">Algebra</a> <a id="2250" href="Base.Homomorphisms.Products.html#2223" class="Bound">α</a><a id="2251" class="Symbol">)</a>
  <a id="2255" class="Symbol">→</a>        <a id="2264" class="Symbol">(∀(</a><a id="2267" href="Base.Homomorphisms.Products.html#2267" class="Bound">i</a> <a id="2269" class="Symbol">:</a> <a id="2271" href="Base.Homomorphisms.Products.html#1595" class="Bound">I</a><a id="2272" class="Symbol">)</a> <a id="2274" class="Symbol">→</a> <a id="2276" href="Base.Homomorphisms.Basic.html#2734" class="Function">hom</a> <a id="2280" class="Symbol">(</a><a id="2281" href="Base.Homomorphisms.Products.html#2234" class="Bound">𝒜</a> <a id="2283" href="Base.Homomorphisms.Products.html#2267" class="Bound">i</a><a id="2284" class="Symbol">)</a> <a id="2286" class="Symbol">(</a><a id="2287" href="Base.Homomorphisms.Products.html#1607" class="Bound">ℬ</a> <a id="2289" href="Base.Homomorphisms.Products.html#2267" class="Bound">i</a><a id="2290" class="Symbol">))</a> <a id="2293" class="Symbol">→</a> <a id="2295" href="Base.Homomorphisms.Basic.html#2734" class="Function">hom</a> <a id="2299" class="Symbol">(</a><a id="2300" href="Base.Algebras.Products.html#1923" class="Function">⨅</a> <a id="2302" href="Base.Homomorphisms.Products.html#2234" class="Bound">𝒜</a><a id="2303" class="Symbol">)(</a><a id="2305" href="Base.Algebras.Products.html#1923" class="Function">⨅</a> <a id="2307" href="Base.Homomorphisms.Products.html#1607" class="Bound">ℬ</a><a id="2308" class="Symbol">)</a>

 <a id="2312" href="Base.Homomorphisms.Products.html#2200" class="Function">⨅-hom</a> <a id="2318" href="Base.Homomorphisms.Products.html#2318" class="Bound">fe</a> <a id="2321" href="Base.Homomorphisms.Products.html#2321" class="Bound">𝒜</a> <a id="2323" href="Base.Homomorphisms.Products.html#2323" class="Bound">𝒽</a> <a id="2325" class="Symbol">=</a> <a id="2327" class="Symbol">(λ</a> <a id="2330" href="Base.Homomorphisms.Products.html#2330" class="Bound">x</a> <a id="2332" href="Base.Homomorphisms.Products.html#2332" class="Bound">i</a> <a id="2334" class="Symbol">→</a> <a id="2336" href="Overture.Basic.html#4325" class="Function Operator">∣</a> <a id="2338" href="Base.Homomorphisms.Products.html#2323" class="Bound">𝒽</a> <a id="2340" href="Base.Homomorphisms.Products.html#2332" class="Bound">i</a> <a id="2342" href="Overture.Basic.html#4325" class="Function Operator">∣</a> <a id="2344" class="Symbol">(</a><a id="2345" href="Base.Homomorphisms.Products.html#2330" class="Bound">x</a> <a id="2347" href="Base.Homomorphisms.Products.html#2332" class="Bound">i</a><a id="2348" class="Symbol">))</a> <a id="2351" href="Agda.Builtin.Sigma.html#235" class="InductiveConstructor Operator">,</a> <a id="2353" class="Symbol">λ</a> <a id="2355" href="Base.Homomorphisms.Products.html#2355" class="Bound">𝑓</a> <a id="2357" href="Base.Homomorphisms.Products.html#2357" class="Bound">𝒶</a> <a id="2359" class="Symbol">→</a> <a id="2361" href="Base.Homomorphisms.Products.html#2318" class="Bound">fe</a> <a id="2364" class="Symbol">λ</a> <a id="2366" href="Base.Homomorphisms.Products.html#2366" class="Bound">i</a> <a id="2368" class="Symbol">→</a> <a id="2370" href="Overture.Basic.html#4363" class="Function Operator">∥</a> <a id="2372" href="Base.Homomorphisms.Products.html#2323" class="Bound">𝒽</a> <a id="2374" href="Base.Homomorphisms.Products.html#2366" class="Bound">i</a> <a id="2376" href="Overture.Basic.html#4363" class="Function Operator">∥</a> <a id="2378" href="Base.Homomorphisms.Products.html#2355" class="Bound">𝑓</a> <a id="2380" class="Symbol">λ</a> <a id="2382" href="Base.Homomorphisms.Products.html#2382" class="Bound">x</a> <a id="2384" class="Symbol">→</a> <a id="2386" href="Base.Homomorphisms.Products.html#2357" class="Bound">𝒶</a> <a id="2388" href="Base.Homomorphisms.Products.html#2382" class="Bound">x</a> <a id="2390" href="Base.Homomorphisms.Products.html#2366" class="Bound">i</a>
</pre>


#### <a id="projections-out-of-products">Projection out of products</a>

Later we will need a proof of the fact that projecting out of a product algebra
onto one of its factors is a homomorphism.

<pre class="Agda">

 <a id="2617" href="Base.Homomorphisms.Products.html#2617" class="Function">⨅-projection-hom</a> <a id="2634" class="Symbol">:</a> <a id="2636" class="Symbol">(</a><a id="2637" href="Base.Homomorphisms.Products.html#2637" class="Bound">i</a> <a id="2639" class="Symbol">:</a> <a id="2641" href="Base.Homomorphisms.Products.html#1595" class="Bound">I</a><a id="2642" class="Symbol">)</a> <a id="2644" class="Symbol">→</a> <a id="2646" href="Base.Homomorphisms.Basic.html#2734" class="Function">hom</a> <a id="2650" class="Symbol">(</a><a id="2651" href="Base.Algebras.Products.html#1923" class="Function">⨅</a> <a id="2653" href="Base.Homomorphisms.Products.html#1607" class="Bound">ℬ</a><a id="2654" class="Symbol">)</a> <a id="2656" class="Symbol">(</a><a id="2657" href="Base.Homomorphisms.Products.html#1607" class="Bound">ℬ</a> <a id="2659" href="Base.Homomorphisms.Products.html#2637" class="Bound">i</a><a id="2660" class="Symbol">)</a>
 <a id="2663" href="Base.Homomorphisms.Products.html#2617" class="Function">⨅-projection-hom</a> <a id="2680" class="Symbol">=</a> <a id="2682" class="Symbol">λ</a> <a id="2684" href="Base.Homomorphisms.Products.html#2684" class="Bound">x</a> <a id="2686" class="Symbol">→</a> <a id="2688" class="Symbol">(λ</a> <a id="2691" href="Base.Homomorphisms.Products.html#2691" class="Bound">z</a> <a id="2693" class="Symbol">→</a> <a id="2695" href="Base.Homomorphisms.Products.html#2691" class="Bound">z</a> <a id="2697" href="Base.Homomorphisms.Products.html#2684" class="Bound">x</a><a id="2698" class="Symbol">)</a> <a id="2700" href="Agda.Builtin.Sigma.html#235" class="InductiveConstructor Operator">,</a> <a id="2702" class="Symbol">λ</a> <a id="2704" href="Base.Homomorphisms.Products.html#2704" class="Bound">_</a> <a id="2706" href="Base.Homomorphisms.Products.html#2706" class="Bound">_</a> <a id="2708" class="Symbol">→</a> <a id="2710" href="Agda.Builtin.Equality.html#207" class="InductiveConstructor">refl</a>

</pre>

We could prove a more general result involving projections onto multiple factors,
but so far the single-factor result has sufficed.

---------------------------------

<span style="float:left;">[← Base.Homomorphisms.Kernels](Base.Homomorphisms.Kernels.html)</span>
<span style="float:right;">[Base.Homomorphisms.Noether →](Base.Homomorphisms.Noether.html)</span>

{% include UALib.Links.md %}
