.. _birkhoffs-hsp-theorem:

======================
Birkhoff's HSP Theorem
======================

Let :math:`Ïƒ = (F, Ï)` be a signature.

An **identity in the signature** Ïƒ is an ordered pair of terms, written :math:`p â‰ˆ q`, from :math:`T_Ïƒ (X_Ï‰)`.

Let :math:`ğ€ = âŸ¨A, F^{ğ€}âŸ©` be an algebra of signature :math:`S`.

We say that ğ€ satisfies :math:`p â‰ˆ q`, and write :math:`ğ€ âŠ§ p â‰ˆ q`, if :math:`p^{ğ€} = q^{ğ€}`.

If ğ’¦ is a class of algebras of signature Ïƒ, we write :math:`ğ’¦ âŠ§ p \approx q` if :math:`âˆ€ ğ€ âˆˆ ğ’¦`, :math:`ğ€ âŠ§ p â‰ˆ q`.

Finally, if Î£ is a set of equations, we write :math:`ğ’¦ âŠ§ Î£` if every member of ğ’¦ satisfies every member of Î£.

Let ğ’¦ be a class of algebras and Î£ a set of equations in the signature Ïƒ. We define :math:`\mathrm{Id}(ğ’¦) = \{p â‰ˆ q : ğ’¦ âŠ§ p â‰ˆ q\}`
and :math:`\mathrm{Mod}(Î£) = \{ ğ€ : ğ€ âŠ§ Î£ \}`.

Classes of the form :math:`\mathrm{Mod}(Î£)` are called **equational classes**, and :math:`Î£` is called an **equational base** or an **axiomatization** of the class.

:math:`\mathrm{Mod}(Î£)` is called the class of **models** of Î£.

Dually, a set of identities of the form :math:`\mathrm{Id}(ğ’¦)` is called an **equational theory**.

.. _a-variety-of-facts:

A variety of theorems
---------------------

.. _fact-m1:

.. proof:theorem::

   For every class ğ’¦, each of the classes :math:`ğ–²(ğ’¦)`, :math:`ğ–§(ğ’¦)`, :math:`ğ–¯(ğ’¦)`, and :math:`ğ•(ğ’¦)` satisfies exactly the same identities as does ğ’¦.

   *Proof*. Exercise.

   .. _fact-m2:

.. proof:theorem:: 

   :math:`ğ’¦ âŠ§ p â‰ˆ q` if and only if for every :math:`ğ€ âˆˆ ğ’¦` and every :math:`h âˆˆ \mathrm{Hom}(ğ“(X_Ï‰), ğ€)`, we have :math:`h(p) = h(q)`.

   .. container:: toggle
 
      .. container:: header
 
         *Proof*.
      
      First assume that :math:`ğ’¦ âŠ§ p â‰ˆ q`. Fix :math:`ğ€âˆˆ ğ’¦` and :math:`h âˆˆ \mathrm{Hom}(ğ“(X_Ï‰), ğ€)`.
      
      Then :math:`ğ€ âŠ§ p â‰ˆ q âŸ¹ p^{ğ€} = q^{ğ€} âŸ¹ p^{ğ€}(h(x_1), \dots, h(x_n)) = q^{ğ€}(h(x_1), \dots, h(x_n))`.
      
      Since :math:`h` is a homomorphism, we obtain :math:`h(p^{ğ€}(x_1, \dots, x_n)) = h(q^{ğ€}(x_1, \dots, x_n))`, i.e., :math:`h(p) = h(q)`.

      To prove the converse we must fix a :math:`ğ€ \in ğ’¦` and :math:`a_1, \dots, a_n âˆˆ A` and show that :math:`p^{ğ€}(x_1, \dots, x_n) = q^{ğ€}(x_1, \dots, x_n)`.
   
      Let :math:`h_0 : X_Ï‰ â†’ A` be a function with :math:`h_0(x_i) = a_i` for :math:`i â‰¤ n`.
      
      By Thm.Â 4.21 in :cite:`Bergman:2012`, :math:`h_0` extends to a homomorphism :math:`h` from :math:`ğ“(X_Ï‰)` to :math:`(A, f^A)`.
      
      By assumption :math:`h(p) = h(q)`. Since :math:`h(p) = h(p^{ğ€}(x_1, \dots, x_n)) = p^{ğ€}(h(x_1), \dots, h(x_n)) = p^{ğ€}(a_1,\dots, a_n)` (and similarly for :math:`q`) the result follows.

   .. _fact-m3:

.. proof:theorem:: 

   Let ğ’¦ be a class of algebras and :math:`p â‰ˆ q` an equation. The following are equivalent.

     #. :math:`ğ’¦ âŠ§ p â‰ˆ q`.

     #. :math:`(p, q)` belongs to the congruence :math:`Î»_{ğ’¦}` on :math:`ğ“(X_Ï‰)`.

     #. :math:`ğ…_{ğ’¦}(X_Ï‰) âŠ§ p â‰ˆ q`.

   .. container:: toggle
 
      .. container:: header
 
         *Proof*.
      
      We shall show (a) âŸ¹ (c) âŸ¹ (b) âŸ¹ (a). 
      
      Throughout the proof we write ğ… for :math:`ğ…_{ğ’¦}(X_Ï‰)`, ğ“ for :math:`ğ“(X_Ï‰)` and :math:`Î»` for :math:`Î»_{ğ’¦}`.

      Recall that :math:`ğ… = ğ“/Î» âˆˆ ğ–² ğ–¯ (ğ’¦)`.
      
      From (a) and LemmaÂ 4.36 of :cite:`Bergman:2012` we have :math:`ğ–² ğ–¯ (ğ’¦) âŠ§ p â‰ˆ q`. Thus (c) holds.

      From (c), :math:`p^{ğ…}([x_1], \dots, [x_n]) = q^{ğ…}([x_1], \dots, [x_n])`, where :math:`[x_i] = x_i/Î»`.
      
      From the definition of ğ…, :math:`p^{ğ“}(x_1, \dots, x_n) â‰¡_Î» q^{ğ“}(x_1, \dots, x_n)`, from which (b) follows since :math:`p = p^{ğ“}(x_1, \dots, x_n)` and :math:`q = q^{ğ“}(x_1, \dots, x_n)`.

      Finally assume (b). We wish to apply LemmaÂ 4.37 of :cite:`Bergman:2012`.
      
      Let :math:`ğ€ âˆˆ ğ’¦` and :math:`h âˆˆ \mathrm{Hom}(ğ“, ğ€)`.
      
      Then :math:`ğ“/\ker h âˆˆ ğ–² (ğ€) âŠ† ğ–²(ğ’¦)` so :math:`\ker h âŠ‡ Î»`.  Thus, (b) implies :math:`h(p) = h(q)` hence (a) holds, completing the proof.

The last result tells us that we can determine whether an identity is true in a variety by consulting a particular algebra, namely :math:`ğ…(X_Ï‰)`. Sometimes it is convenient to work with algebras free on other generating sets besides :math:`X_Ï‰`. The following corollary takes care of that for us.

.. _fact-m4:

.. proof:theorem:: 

   Let :math:`ğ’¦` be a class of algebras, :math:`p` and :math:`q` :math:`n`-ary terms, :math:`Y` a set and :math:`y_1, \dots, y_n` distinct elements of :math:`Y`. Then :math:`ğ’¦ âŠ§ p â‰ˆ q` if and only if
   :math:`p^{ğ…_{ğ’¦}(Y)}(y_1, \dots, y_n) = q^{ğ…_{ğ’¦}(Y)}(y_1, \dots, y_n)`. In particular, :math:`ğ’¦ âŠ§ p â‰ˆ q` if and only if :math:`ğ…_{ğ’¦}(X_n) âŠ§ p â‰ˆ q`.

   .. container:: toggle
 
      .. container:: header
 
         *Proof*.
      
      Since :math:`ğ…_{ğ’¦}(Y) âˆˆ ğ–² ğ–¯ (ğ’¦)`, the left-to-right direction uses the same argument as in TheoremÂ 4.38 of :cite:`Bergman:2012`. (See :ref:`Fact 3 <fact-m3>` above.)
      
      So assume that :math:`p^{ğ…_{ğ’¦}(Y)}(y_1, \dots, y_n) = q^{ğ…_{ğ’¦}(Y)}(y_1, \dots, y_n)`.
      
      To show that :math:`ğ’¦ âŠ§ p â‰ˆ q`, let :math:`ğ€ = âŸ¨ A, f^{ğ€} âŸ© âˆˆ ğ’¦` and :math:`a_1, \dots, a_n âˆˆ A`. We must show :math:`p^{ğ€}(a_1, \dots, a_n) = q^{ğ€}(a_1, \dots, a_n)`.

      There is a homomorphism :math:`h : ğ…_{ğ’¦}(Y) â†’ (A, f^A)` such that :math:`h(y_i) = a_i` for :math:`i â‰¤ n`. Then

      .. math:: p^{ğ€}(a_1, \dots, a_n) &= p^{ğ€}(h (y_1), \dots, h (y_n)) = h(p^{ğ…_ğ’¦(Y)}(y_1, \dots, y_n))\\
                                       &= h(q^{ğ…_ğ’¦(Y)}(y_1, \dots, y_n)) = q^{ğ€}(h(y_1), \dots, h(y_n))\\
                                       &= q^{ğ€}(a_1, \dots, a_n).

      It now follows from :ref:`Fact 1 <fact-m1>` that every equational class is a variety. The converse is **Birkhoff's HSP Theorem**.

.. _the-hsp-theorem:

The HSP theorem
---------------

The following is Birkhoff's celebrated HSP theorem. (See also :cite:`Bergman:2012`, Thm 4.41.)

.. proof:theorem:: 

   Every variety is an equational class.

   .. container:: toggle
 
      .. container:: header
 
         *Proof*.
      
      Let ğ’² be a variety. We must find a set of equations that axiomatizes ğ’². The obvious choice is to use the set of all equations that hold in ğ’².

      To this end, take :math:`Î£ = \mathrm{Id}(ğ’²)`. Let :math:`ğ’²^â€  := \mathrm{Mod}(Î£)`.  
  
      Clearly, :math:`ğ’² âŠ† ğ’²^â€ `. We shall prove the reverse inclusion.

      Let :math:`ğ€ âˆˆ ğ’²^â€ ` and :math:`Y` a set of cardinality :math:`\max(|A|, Ï‰)`. *Choose* a surjection :math:`h_0 : Y â†’ A`. [1]_
  
      By :ref:`TheoremÂ 4.21 <thm-4-21>`, :math:`h_0` extends to a (surjective) homomorphism :math:`h : ğ“(Y) â†’ ğ€`.

      Furthermore, since :math:`ğ…_{ğ’²}(Y) = ğ“(Y)/Î˜_{ğ’²}`, there is a surjective homomorphism :math:`g : ğ“(Y) â†’ ğ…_{ğ’²}`. [2]_

      We claim that :math:`\ker g âŠ† \ker h`. If the claim is true then by LemmaÂ [ex:1.26.8] there is a map :math:`f : ğ…_{ğ’²}(Y) â†’ ğ€` such that :math:`f âˆ˜ g = h`.
   
      Since :math:`h` is surjective, so is :math:`f`. Hence :math:`ğ€ âˆˆ ğ–§ (ğ…_{ğ’²}(Y)) âŠ† ğ’²` completing the proof.

Let :math:`u,v âˆˆ T(Y)` and assume that :math:`g(u) = g(v)`. Since :math:`ğ“(Y)` is generated by :math:`Y`, by :ref:`TheoremÂ 4.21 <thm-4-21>`, there is an integer :math:`n`, terms :math:`p, q âˆˆ T(X_n)`, and :math:`y_1, \dots, y_n âˆˆ Y` such that :math:`u = p^{ğ“(Y)}(y_1, \dots, y_n)` and :math:`v = q^{ğ“(Y)}(y_1,\dots, y_n)`, by TheoremÂ [thm:4.32].

Applying the homomorphism :math:`g`,

.. math:: p^{ğ…_{ğ’²}(Y)}(y_1, \dots, y_n) = g(u) = g(v) = q^{ğ…_{ğ’²}(Y)}(y_1,\dots, y_n).

Then by :ref:`Fact 4 <fact-m4>` above (CorollaryÂ 4.39 of :cite:`Bergman:2012`), we have :math:`ğ’² âŠ§ p â‰ˆ q`, hence :math:`(p â‰ˆ q) \in Î£`.

Since :math:`ğ€ âˆˆ ğ’²^â€  = \mathrm{Mod}(Î£)`, we obtain :math:`ğ€ âŠ§ p â‰ˆ q`. Therefore,

.. math:: h(u) = p^{ğ€}(h_0(y_1), \dots, h_0(y_n)) = q^{ğ€}(h_0(y_1), \dots, h_0(y_n)) = h(v),

as desired.

---------------------------

.. rubric:: Footnotes

.. [1]
   **AoC**. It seems we need the Axiom of Choice here.

.. [2]
   **AoC**. *ditto*