.. FILE: terms.lagda.rst
.. AUTHOR: William DeMeo and Siva Somayyajula
.. DATE: 20 Feb 2020
.. UPDATE: 27 Jun 2020

.. open import UF-Extensionality using (propext; dfunext; funext; _âˆˆ_; global-funext; hfunext; intensionality)
.. open import Relation.Unary using (Pred)

.. _types for terms:

===============
Types for Terms
===============

Preliminaries
-------------

As usual, we start with the imports we will need below.

::

   {-# OPTIONS --without-K --exact-split --safe #-}

   open import prelude
   open import basic using (Signature; Algebra; Î ')
   open import homomorphisms using (HOM; Hom; hom)
   open import relations using (Con; compatible-fun)

Terms in Agda
------------------------

We developed the notion of a term in a signature informally in :numref:`terms`.  Here we formalize this concept in an Agda module called ``terms``. We start by defining a datatype called ``Term`` which, not surprisingly, represents the type of terms.

::

   module terms {S : Signature ğ“ ğ“¥} where  -- ğ“ âŠ” ğ“¥ âŠ” ğ“¤

   module _ where
     data Term {X : ğ“§ Ì‡}  :  ğ“ âŠ” ğ“¥ âŠ” ğ“§ Ì‡  where
       generator : X â†’ Term {X = X}
       node : ( ğ“¸ : âˆ£ S âˆ£ )  â†’  ( ğ’• : âˆ¥ S âˆ¥ ğ“¸ â†’ Term {X = X} )  â†’  Term {X = X}

     open Term

The term algebra
~~~~~~~~~~~~~~~~~~

The term algebra was described informally in :numref:`terms`.  Here is how we implement this important algebra in Agda.

::

     ğ”‰ : {X : ğ“§ Ì‡} â†’ Algebra (ğ“ âŠ” ğ“¥ âŠ” ğ“§) S
     ğ”‰ {X = X} = Term{X = X} , node

The universal property of ğ”‰
~~~~~~~~~~~~~~~~~~~~~~~~~~~

We prove

  #. every `â„ : X â†’ âˆ¥ ğ‘¨ âˆ¥  lifts to a hom from ğ”‰ to ğ‘¨.
  #. the induced homomorphism is unique.

::

   module _ {ğ‘¨ : Algebra ğ“¤ S} { X : ğ“§ Ì‡} where

    --1.a. Every map  (X â†’ A)  "lifts".
    free-lift : (h : X â†’ âˆ£ ğ‘¨ âˆ£)  â†’   âˆ£ ğ”‰ âˆ£ â†’ âˆ£ ğ‘¨ âˆ£
    free-lift h (generator x) = h x
    free-lift h (node ğ“¸ args) = (âˆ¥ ğ‘¨ âˆ¥ ğ“¸) Î»{i â†’ free-lift  h (args i)}

    --I. Extensional proofs (using hom's)
    --1.b.' The lift is (extensionally) a hom
    lift-hom : (h : X â†’ âˆ£ ğ‘¨ âˆ£) â†’  hom ğ”‰ ğ‘¨
    lift-hom h = free-lift h , Î» ğ“¸ ğ’‚ â†’ ap (âˆ¥ ğ‘¨ âˆ¥ _) (refl _)

    --2.' The lift to  (free â†’ A)  is (extensionally) unique.
    free-unique : funext ğ“¥ ğ“¤ â†’ ( f g : hom (ğ”‰ {X = X}) ğ‘¨ )
     â†’             ( âˆ€ x  â†’  âˆ£ f âˆ£ (generator x) â‰¡ âˆ£ g âˆ£ (generator x) )
     â†’             (t : Term )
                   ---------------------------
     â†’              âˆ£ f âˆ£ t â‰¡ âˆ£ g âˆ£ t

    free-unique fe f g p (generator x) = p x
    free-unique fe f g p (node ğ“¸ args) =
       (âˆ£ f âˆ£)(node ğ“¸ args)            â‰¡âŸ¨ âˆ¥ f âˆ¥ ğ“¸ args âŸ©
       (âˆ¥ ğ‘¨ âˆ¥ ğ“¸)(Î» i â†’ âˆ£ f âˆ£ (args i))  â‰¡âŸ¨ ap (âˆ¥ ğ‘¨ âˆ¥ _) (fe (Î» i â†’ free-unique fe f g p (args i))) âŸ©
       (âˆ¥ ğ‘¨ âˆ¥ ğ“¸)(Î» i â†’ âˆ£ g âˆ£ (args i))  â‰¡âŸ¨ (âˆ¥ g âˆ¥ ğ“¸ args)â»Â¹ âŸ©
       âˆ£ g âˆ£ (node ğ“¸ args)             âˆ


Intensional proofs
~~~~~~~~~~~~~~~~~~~

Here we use `HOM` instead of `hom`. N.B. using this "intensional" definition of hom, we don't need function extensionality to prove uniqueness of the hom extension.

::

    --1.b. that free-lift is (intensionally) a hom.
    lift-HOM : (h : X â†’ âˆ£ ğ‘¨ âˆ£) â†’  HOM ğ”‰ ğ‘¨
    lift-HOM  h = free-lift h , refl _

    --2. The lift to  (free â†’ A)  is (intensionally) unique.

    free-intensionally-unique : funext ğ“¥ ğ“¤ â†’ ( f g : HOM (ğ”‰{X = X}) ğ‘¨ )
     â†’             ( âˆ£ f âˆ£ âˆ˜ generator ) â‰¡ ( âˆ£ g âˆ£ âˆ˜ generator )
     â†’             (t : Term)
                   --------------------------------
     â†’              âˆ£ f âˆ£ t â‰¡ âˆ£ g âˆ£ t

    free-intensionally-unique fe f g p (generator x) = intensionality p x
    free-intensionally-unique fe f g p (node ğ“¸ args) =
       ( âˆ£ f âˆ£ )(node ğ“¸ args)       â‰¡âŸ¨ ap (Î» - â†’ - ğ“¸ args) âˆ¥ f âˆ¥  âŸ©
       (âˆ¥ ğ‘¨ âˆ¥ ğ“¸) ( âˆ£ f âˆ£ âˆ˜ args )   â‰¡âŸ¨ ap (âˆ¥ ğ‘¨ âˆ¥ _) (fe (Î» i â†’ free-intensionally-unique fe f g p (args i)) ) âŸ©
       (âˆ¥ ğ‘¨ âˆ¥ ğ“¸) ( âˆ£ g âˆ£ âˆ˜ args )   â‰¡âŸ¨ (ap (Î» - â†’ - ğ“¸ args) âˆ¥ g âˆ¥ ) â»Â¹ âŸ©
       âˆ£ g âˆ£ (node ğ“¸ args)         âˆ

Interpretations
-------------------

Syntactic sugar:  `ğ“¸ Ì‚ ğ‘¨  â‰¡  âŸ¦ ğ‘¨ âŸ§ ğ“¸`

Before proceding, we define some syntactic sugar that allows us to replace `âŸ¦ ğ‘¨ âŸ§ ğ“¸` with (the more standard-looking) `ğ“¸ Ì‚ ğ‘¨`.

::

   _Ì‚_ :  (ğ“¸ : âˆ£ S âˆ£ ) â†’ (ğ‘¨ : Algebra ğ“¤ S)
    â†’       ( âˆ¥ S âˆ¥ ğ“¸  â†’  âˆ£ ğ‘¨ âˆ£ ) â†’ âˆ£ ğ‘¨ âˆ£
   ğ“¸ Ì‚ ğ‘¨ = Î» x â†’ (âˆ¥ ğ‘¨ âˆ¥ ğ“¸) x

We can now write `ğ“¸ Ì‚ ğ‘¨` for the interpretation of the basic operation `ğ“¸` in the algebra `ğ‘¨`. N.B. below, we will write `ğ’• Ì‡ ğ‘¨` for the interpretation of a *term* `ğ’•` in `ğ‘¨`.

(todo: probably we should figure out how to use the same notation for both, if possible)

Interpretation of terms
~~~~~~~~~~~~~~~~~~~~~~~~~~~~~~~

(cf Def 4.31 of Bergman)

Let `ğ’• : Term` be a term and `ğ‘¨` an S-algebra. We define the n-ary operation `ğ’• Ì‡ ğ‘¨` on `ğ‘¨` by structural recursion on `ğ’•`.

  #. if `ğ’• = x âˆˆ X` (a variable) and `ğ’‚ : X â†’ âˆ£ ğ‘¨ âˆ£` is a tuple from `A`, then `(t Ì‡ ğ‘¨) ğ’‚ = ğ’‚ x`.
  #. if `ğ’• = ğ“¸ args`, where `ğ“¸ âˆˆ âˆ£ S âˆ£` is an op symbol and `args : âŸ¦ S âŸ§ ğ“¸ â†’ Term` is an (`âŸ¦ S âŸ§ ğ“¸`)-tuple of terms and `ğ’‚ : X â†’ âˆ£ A âˆ£` is a tuple from `A`, then `(ğ’• Ì‡ ğ‘¨) ğ’‚ = ((ğ“¸ args) Ì‡ ğ‘¨) ğ’‚ = (ğ“¸ Ì‚ ğ‘¨) Î»{ i â†’ ((args i) Ì‡ ğ‘¨) ğ’‚ }`

::

   _Ì‡_ : { X : ğ“§ Ì‡ } â†’ Term{X = X}  â†’ (ğ‘¨ : Algebra ğ“¤ S) â†’  ( X â†’ âˆ£ ğ‘¨ âˆ£ ) â†’ âˆ£ ğ‘¨ âˆ£
   ((generator x)Ì‡ ğ‘¨) ğ’‚ = ğ’‚ x
   ((node ğ“¸ args)Ì‡ ğ‘¨) ğ’‚ = (ğ“¸ Ì‚ ğ‘¨) Î»{x â†’ (args x Ì‡ ğ‘¨) ğ’‚ }

   ğ”‰-interp : { X : ğ“§ Ì‡ } â†’ Term{X = X} â†’  ( X â†’ Term{X = X} ) â†’ Term{X = X}
   ğ”‰-interp (generator x) ğ’‚ = ğ’‚ x
   ğ”‰-interp (node ğ“¸ args) ğ’‚ = node ğ“¸ (Î» (i : âˆ¥ S âˆ¥ ğ“¸ ) â†’   (ğ”‰-interp (args i) ğ’‚) )

   interp-prod : funext ğ“¥ ğ“¤ â†’ { X : ğ“§ Ì‡}{I : ğ“¤ Ì‡} (p : Term{X = X})  (ğ“ : I â†’ Algebra ğ“¤ S) ( x : X â†’ âˆ€ i â†’ âˆ£ (ğ“ i) âˆ£ )
    â†’              (p Ì‡ (Î ' ğ“)) x  â‰¡   (Î» i â†’ (p Ì‡ ğ“ i) (Î» j -> x j i))
   interp-prod fe (generator xâ‚) ğ“ x = refl _
   interp-prod fe (node ğ“¸ ğ’•) ğ“ x =
     let IH = Î» xâ‚ â†’ interp-prod fe (ğ’• xâ‚) ğ“ x in
         âˆ¥ Î ' ğ“ âˆ¥ ğ“¸ (Î» xâ‚ â†’ (ğ’• xâ‚ Ì‡ Î ' ğ“) x)                         â‰¡âŸ¨ ap (âˆ¥ Î ' ğ“ âˆ¥ ğ“¸ ) (fe IH) âŸ©
         âˆ¥ Î ' ğ“ âˆ¥ ğ“¸ (Î» xâ‚ â†’ (Î» iâ‚ â†’ (ğ’• xâ‚ Ì‡ ğ“ iâ‚) (Î» jâ‚ â†’ x jâ‚ iâ‚))) â‰¡âŸ¨ refl _ âŸ©   -- refl _ âŸ©
         (Î» iâ‚ â†’ âˆ¥ ğ“ iâ‚ âˆ¥ ğ“¸ (Î» xâ‚ â†’ (ğ’• xâ‚ Ì‡ ğ“ iâ‚) (Î» jâ‚ â†’ x jâ‚ iâ‚)))  âˆ

   interp-prod2 : global-dfunext â†’ { X : ğ“§ Ì‡}{I : ğ“¤ Ì‡} (p : Term{X = X}) ( A : I â†’ Algebra ğ“¤ S )
    â†’              (p Ì‡ Î ' A)  â‰¡  Î» (args : X â†’ âˆ£ Î ' A âˆ£ ) â†’ ( Î» áµ¢ â†’ (p Ì‡ A áµ¢ ) ( Î» x â†’ args x áµ¢ ) )
   interp-prod2 fe (generator xâ‚) A = refl _
   interp-prod2 fe {X = X} (node ğ“¸ ğ’•) A = fe Î» ( tup : X â†’ âˆ£ Î ' A âˆ£ ) â†’
     let IH = Î» x â†’ interp-prod fe (ğ’• x) A  in
     let tá´¬ = Î» z â†’ ğ’• z Ì‡ Î ' A in
       ( ğ“¸ Ì‚ Î ' A )  ( Î» s â†’ tá´¬ s tup )                 â‰¡âŸ¨ refl _ âŸ©
       âˆ¥ Î ' A âˆ¥ ğ“¸ ( Î» s â†’  tá´¬ s tup )                    â‰¡âŸ¨ ap ( âˆ¥ Î ' A âˆ¥ ğ“¸ ) (fe  Î» x â†’ IH x tup) âŸ©
       âˆ¥ Î ' A âˆ¥ ğ“¸ (Î» s â†’ (Î» â±¼ â†’ (ğ’• s Ì‡ A â±¼ ) (Î» â„“ â†’ tup â„“ â±¼ )))    â‰¡âŸ¨ refl _ âŸ©
       (Î» áµ¢ â†’ (ğ“¸ Ì‚ A áµ¢ ) (Î» s â†’ (ğ’• s Ì‡ A áµ¢ ) (Î» â„“ â†’ tup â„“ áµ¢ )))       âˆ

.. _obs 10 agda:

Compatibility of homs and terms
~~~~~~~~~~~~~~~~~~~~~~~~~~~~~~~~~~

In this section we present the formal proof of the fact that homomorphisms commute with terms.  More precisely, if ğ‘¨ and ğ‘© are ğ‘†-algebras, ğ‘“ : ğ‘¨ â†’ ğ‘© a homomorphism, and ğ‘¡ a term in the language of ğ‘†, then for all ğ’‚ : X â†’ âˆ£ ğ‘¨ âˆ£ we have :math:`ğ‘“ (ğ‘¡^ğ‘¨ ğ’‚) = ğ‘¡^ğ‘© (ğ‘“ âˆ˜ ğ’‚)`.


::

   -- Proof of 1. (homomorphisms commute with terms).
   comm-hom-term : global-dfunext
    â†’              {X : ğ“§ Ì‡}(ğ‘¨ : Algebra ğ“¤ S) (ğ‘© : Algebra ğ“¦ S)
                   (g : HOM ğ‘¨ ğ‘©) (ğ’• : Term{X = X})
                  ---------------------------------------------
    â†’              âˆ£ g âˆ£ âˆ˜ (ğ’• Ì‡ ğ‘¨) â‰¡ (ğ’• Ì‡ ğ‘©) âˆ˜ (Î» ğ’‚ â†’ âˆ£ g âˆ£ âˆ˜ ğ’‚ )
   comm-hom-term gfe ğ‘¨ ğ‘© g (generator x) = refl _
   comm-hom-term gfe {X = X}ğ‘¨ ğ‘© g (node ğ“¸ args) = Î³
    where
     Î³ : âˆ£ g âˆ£ âˆ˜ (Î» ğ’‚ â†’ (ğ“¸ Ì‚ ğ‘¨) (Î» i â†’ (args i Ì‡ ğ‘¨) ğ’‚))     â‰¡ (Î» ğ’‚ â†’ (ğ“¸ Ì‚ ğ‘©)(Î» i â†’ (args i Ì‡ ğ‘©) ğ’‚)) âˆ˜ _âˆ˜_ âˆ£ g âˆ£
     Î³ =  âˆ£ g âˆ£ âˆ˜ (Î» ğ’‚ â†’ (ğ“¸ Ì‚ ğ‘¨) (Î» i â†’ (args i Ì‡ ğ‘¨) ğ’‚))    â‰¡âŸ¨ ap (Î» - â†’ (Î» ğ’‚ â†’ - ğ“¸ (Î» i â†’ (args i Ì‡ ğ‘¨) ğ’‚))) âˆ¥ g âˆ¥ âŸ©
         (Î» ğ’‚ â†’ (ğ“¸ Ì‚ ğ‘©)(âˆ£ g âˆ£ âˆ˜ (Î» i â†’  (args i Ì‡ ğ‘¨) ğ’‚)))   â‰¡âŸ¨ refl _ âŸ©
         (Î» ğ’‚ â†’ (ğ“¸ Ì‚ ğ‘©)(Î» i â†’ âˆ£ g âˆ£ ((args i Ì‡ ğ‘¨) ğ’‚)))      â‰¡âŸ¨ ap (Î» - â†’ (Î» ğ’‚ â†’ (ğ“¸ Ì‚ ğ‘©)(- ğ’‚))) ih âŸ©
         ((Î» ğ’‚ â†’ (ğ“¸ Ì‚ ğ‘©)(Î» i â†’ (args i Ì‡ ğ‘©) ğ’‚)) âˆ˜ _âˆ˜_ âˆ£ g âˆ£) âˆ
       where
        IH : (ğ’‚ : X â†’ âˆ£ ğ‘¨ âˆ£)(i : âˆ¥ S âˆ¥ ğ“¸) â†’ ((âˆ£ g âˆ£ âˆ˜ (args i Ì‡ ğ‘¨)) ğ’‚) â‰¡ (((args i Ì‡ ğ‘©) âˆ˜ _âˆ˜_ âˆ£ g âˆ£) ğ’‚)
        IH ğ’‚ i = intensionality (comm-hom-term gfe ğ‘¨ ğ‘© g (args i)) ğ’‚

        IH' : (i : âˆ¥ S âˆ¥ ğ“¸) â†’ ((âˆ£ g âˆ£ âˆ˜ (args i Ì‡ ğ‘¨))) â‰¡ ((args i Ì‡ ğ‘©) âˆ˜ _âˆ˜_ âˆ£ g âˆ£)
        IH' i = (comm-hom-term gfe ğ‘¨ ğ‘© g (args i))

        ih : (Î» ğ’‚ â†’ (Î» i â†’ âˆ£ g âˆ£ ((args i Ì‡ ğ‘¨) ğ’‚))) â‰¡ (Î» ğ’‚ â†’ (Î» i â†’ ((args i Ì‡ ğ‘©) âˆ˜ _âˆ˜_ âˆ£ g âˆ£) ğ’‚))
        ih = gfe Î» ğ’‚ â†’ gfe Î» i â†’ IH ğ’‚ i

        ih' : (Î» i â†’ âˆ£ g âˆ£ âˆ˜ (args i Ì‡ ğ‘¨)) â‰¡ (Î» i â†’ ((args i Ì‡ ğ‘©) âˆ˜ _âˆ˜_ âˆ£ g âˆ£))
        ih' = gfe Î» i â†’ IH' i


.. _obs 11 agda:

Compatibility of congruences and terms
~~~~~~~~~~~~~~~~~~~~~~~~~~~~~~~~~~~~~~~~~~~

Here we present an Agda proof of the fact that terms respect congruences. More precisely, we show that for every term ğ‘¡, every Î¸ âˆˆ Con(ğ‘¨), and all tuples ğ’‚, ğ’ƒ : ğ‘‹ â†’ ğ‘¨, we have (âˆ€ i, ğ’‚(i) Î¸ ğ’ƒ(i)) â†’ (t^ğ‘¨ ğ’‚) Î¸ (t^ğ‘¨ ğ’ƒ).

::

   compatible-term : {X : ğ“§ Ì‡}(ğ‘¨ : Algebra ğ“¤ S)
                     ( ğ’• : Term{X = X} ) (Î¸ : Con ğ‘¨)
                    ----------------------------------
    â†’                  compatible-fun (ğ’• Ì‡ ğ‘¨) âˆ£ Î¸ âˆ£

   compatible-term ğ‘¨ (generator x) Î¸ p = p x
   compatible-term ğ‘¨ (node ğ“¸ args) Î¸ p = âˆ¥ âˆ¥ Î¸ âˆ¥ âˆ¥ ğ“¸ Î»{ x â†’ (compatible-term ğ‘¨ (args x) Î¸) p }

   -- For proof of 3, see `TermImageSub` in Subuniverse.agda.


Extensional versions
~~~~~~~~~~~~~~~~~~~~~~~~~

::

   -- Proof of 1. (homomorphisms commute with terms).
   comm-hom-term' : global-dfunext --  ğ“¥ ğ“¤
    â†’               {X : ğ“§ Ì‡}(ğ‘¨ : Algebra ğ“¤ S) (ğ‘© : Algebra ğ“¦ S)
    â†’               (g : hom ğ‘¨ ğ‘©) (ğ’• : Term{X = X}) (ğ’‚ : X â†’ âˆ£ ğ‘¨ âˆ£)
                  --------------------------------------------
    â†’               âˆ£ g âˆ£ ((ğ’• Ì‡ ğ‘¨) ğ’‚) â‰¡ (ğ’• Ì‡ ğ‘©) (âˆ£ g âˆ£ âˆ˜ ğ’‚)

   comm-hom-term' fe ğ‘¨ ğ‘© g (generator x) ğ’‚ = refl _
   comm-hom-term' fe ğ‘¨ ğ‘© g (node ğ“¸ args) ğ’‚ =
       âˆ£ g âˆ£ ((ğ“¸ Ì‚ ğ‘¨)  (Î» iâ‚ â†’ (args iâ‚ Ì‡ ğ‘¨) ğ’‚))     â‰¡âŸ¨ âˆ¥ g âˆ¥ ğ“¸ ( Î» r â†’ (args r Ì‡ ğ‘¨) ğ’‚ ) âŸ©
       (ğ“¸ Ì‚ ğ‘©) ( Î» iâ‚ â†’  âˆ£ g âˆ£ ((args iâ‚ Ì‡ ğ‘¨) ğ’‚) )    â‰¡âŸ¨ ap (_ Ì‚ ğ‘©) ( fe (Î» iâ‚ â†’ comm-hom-term' fe ğ‘¨ ğ‘© g (args iâ‚) ğ’‚) ) âŸ©
       (ğ“¸ Ì‚ ğ‘©) ( Î» r â†’ (args r Ì‡ ğ‘©) (âˆ£ g âˆ£ âˆ˜ ğ’‚) )        âˆ


   -- Proof of 2.  (If t : Term, Î¸ : Con A, then a Î¸ b  â†’  t(a) Î¸ t(b). )
   compatible-term' :  {X : ğ“§ Ì‡}(ğ‘¨ : Algebra ğ“¤ S) ( ğ’• : Term{X = X}  ) (Î¸ : Con ğ‘¨)
                            ------------------------------------------------------
    â†’                              compatible-fun (ğ’• Ì‡ ğ‘¨) âˆ£ Î¸ âˆ£

   compatible-term' ğ‘¨ (generator x) Î¸ p = p x
   compatible-term' ğ‘¨ (node ğ“¸ args) Î¸ p = âˆ¥ âˆ¥ Î¸ âˆ¥ âˆ¥ ğ“¸ Î»{ x â†’ (compatible-term' ğ‘¨ (args x) Î¸) p }

For proof of 3, see `TermImageSub` in Subuniverse.agda.

..    #. For every subset Y of A,  Sg ( Y ) = { t (aâ‚, ..., aâ‚™ ) : t âˆˆ T(Xâ‚™), n < Ï‰, aáµ¢ âˆˆ Y, i â‰¤ n}.




------------------

.. include:: hyperlink_references.rst

