--File: free.agda
--Author: William DeMeo and Siva Somayyajula
--Date: 25 Dec 2019
--Updated: 17 Feb 2020

{-# OPTIONS --without-K --exact-split #-}

open import preliminaries
-- open import preliminaries  using (_âŠ_ ; âˆ€-extensionality; âˆ‘; List)
open import basic 

module free  {S : signature} {X : Set} where

open import Level
open import Agda.Builtin.Nat public
  renaming ( Nat to â„•; _-_ to _âˆ¸_; zero to nzero; suc to succ )
open import Data.Product using (Î£; _,_; âˆƒ; Î£-syntax; âˆƒ-syntax; _Ã—_)
open import Relation.Unary hiding (_âŠ†_;_â‡’_)
-- open import Relation.Binary.Core using (IsEquivalence)
--open import Relation.Binary using (IsEquivalence)
import Relation.Binary.PropositionalEquality as Eq
  hiding (setoid; Reveal_Â·_is_;[_];âˆ€-extensionality)
open Eq using (_â‰¡_; refl; cong; sym)
open Eq.â‰¡-Reasoning
open import Function using (_âˆ˜_)
open import Function.Equality renaming (_âˆ˜_ to _âˆ˜â‚›_) hiding (cong)

open import Relation.Nullary using (Â¬_)
open import Relation.Nullary.Negation using ()
  renaming (contradiction to Â¬Â¬-intro)
--  using    ( _+_; _*_ )

-- open import Data.Fin public
--   -- (See "NOTE on Fin" section below)
--   hiding ( _+_; _<_ )
--   renaming ( suc to fsucc; zero to fzero )
--------------------------------------------------------------


----------------------------
-- TERMS in the signature S
----------------------------
open signature


data Term : Set where
  generator : X -> Term
  node : âˆ€ (ğ“¸ : S ğ“•) -> (â„• -> Term) -> Term

open Term

-- map-Term : (Term -> Term) -> Term -> Term
-- map-Term f (generator x) = f (generator x)
-- map-Term f (node ğ“¸ t) = node ğ“¸ (Î» i -> map-Term f (t i))

----------------------------------
-- TERM ALGEBRA (for signature S)
----------------------------------

open algebra
open Term

free : algebra S
free = record { âŸ¦_âŸ§áµ¤ = Term ; _âŸ¦_âŸ§ = node }

--------------------------------------------------------------
-- analogue for setoid-based algebras
open Setoid
open Algebra

Free : Algebra S
Free = record
       { âŸ¦_âŸ§áµ£ = record
               { Carrier = Term
               ; _â‰ˆ_ = _â‰¡_
               ; isEquiv = isequiv
               }
       ; _âŸ¦_âŸ§ = node
       }
       where
         isequiv = record
                   { refl = Î» {x} â†’ refl
                   ; sym = sym
                   ; trans = Î» {i} {j} {k} p q
                              ->  begin
                                    i
                                  â‰¡âŸ¨ p âŸ©
                                    j
                                  â‰¡âŸ¨ q âŸ©
                                    k
                                  âˆ
                   }


-------------------------------------
-- The UNIVERSAL PROPERTY of free

-- We first prove this for algebras whose carriers are mere sets.

-- 1. every h : X -> âŸ¦ A âŸ§áµ¤  lifts to a hom from free to A.
-- 2. the induced hom is unique.

-- PROOF.
-- 1.a. Every map  (X -> A)  "lifts".
free-lift : {A : algebra  S}(h : X -> âŸ¦ A âŸ§áµ¤) -> âŸ¦ free âŸ§áµ¤ -> âŸ¦ A âŸ§áµ¤
free-lift h (generator x) = h x
free-lift {A} h (node ğ“¸ args) = (A âŸ¦ ğ“¸ âŸ§) Î»{i -> free-lift {A} h (args i)}

-- 1.b. The lift is a hom.
open hom
lift-hom : {A : algebra S} (h : X -> âŸ¦ A âŸ§áµ¤) -> hom free A
lift-hom {A} h = record { âŸ¦_âŸ§â‚• = free-lift {A} h; homo = Î» args â†’ refl }

-- 2. The lift to  (free -> A)  is unique.
--    (We need EXTENSIONALITY for this (imported from util.agda))
free-unique : {A : algebra S}
  ->    ( f g : hom free A )
  ->    ( âˆ€ x  ->  âŸ¦ f âŸ§â‚• (generator x) â‰¡ âŸ¦ g âŸ§â‚• (generator x) )
  ->    (t : Term)
       ---------------------------
  ->    âŸ¦ f âŸ§â‚• t â‰¡ âŸ¦ g âŸ§â‚• t

free-unique {A} f g p (generator x) = p x
free-unique {A} f g p (node ğ“¸ args) =
   begin
     âŸ¦ f âŸ§â‚• (node ğ“¸ args)
   â‰¡âŸ¨ homo f args  âŸ©
     (A âŸ¦ ğ“¸ âŸ§) (Î» i -> âŸ¦ f âŸ§â‚• (args i))
   â‰¡âŸ¨ cong ((A âŸ¦_âŸ§)_)
      ( âˆ€-extensionality Î» i -> free-unique f g p (args i) ) âŸ©
     (A âŸ¦ ğ“¸ âŸ§) (Î» i -> âŸ¦ g âŸ§â‚• (args i))
   â‰¡âŸ¨ sym (homo g args) âŸ©
     âŸ¦ g âŸ§â‚• (node ğ“¸ args)
   âˆ



---------------------------------------------------------------
-- SETOID-based analogue
--
-- Next we prove the universal property of Free for algebras
-- whose carriers are setoids.

open Setoid 
Free-Lift : {A : Algebra  S}(h : X -> âˆ¥ âŸ¦ A âŸ§áµ£ âˆ¥) -> âˆ¥ âŸ¦ Free âŸ§áµ£ âˆ¥ -> âˆ¥ âŸ¦ A âŸ§áµ£ âˆ¥
Free-Lift h (generator x) = h x
Free-Lift {A} h (node ğ“¸ args) = (A âŸ¦ ğ“¸ âŸ§) Î» i -> Free-Lift {A} h (args i)

----------------------------------------
-- 1.b. The lift is a hom.
open Hom
Lift-Hom : {A : Algebra S} (h : X -> âˆ¥ âŸ¦ A âŸ§áµ£ âˆ¥) -> Hom Free A
Lift-Hom {A} h = record { âŸ¦_âŸ§â‚• = Free-Lift {A} h; Homo = Î» args â†’ {!!}}
-- Lift-Hom {A} h = record { âŸ¦_âŸ§â‚• = Free-Lift {A} h; Homo = Î» args â†’ refl âŸ¦ A âŸ§áµ£ }

-- 2. The lift to  (free -> A)  is unique.
--    (We need EXTENSIONALITY for this (imported from util.agda))
Free-Unique : {A : Algebra S}
  ->    ( f g : Hom Free A )
  ->    ( âˆ€ x  ->   (âŸ¦ A âŸ§áµ£ â‰ˆ âŸ¦ f âŸ§â‚• (generator x)) (âŸ¦ g âŸ§â‚• (generator x)) )
  ->    (t : Term)
       ---------------------------
  ->    ( âŸ¦ A âŸ§áµ£ â‰ˆ  âŸ¦ f âŸ§â‚• t ) (âŸ¦ g âŸ§â‚• t)
   --   âŸ¦ f âŸ§â‚• (node ğ“¸ args)
Free-Unique = {!!}
--    ( âˆ€-extensionality Î» i -> free-unique f g p (args i) ) âŸ©

--      ( âˆ€-extensionality  ) âŸ©
   -- begin
   --   âŸ¦ f âŸ§â‚• (node ğ“¸ args)
   -- â‰¡âŸ¨ Homo f args  âŸ©
   --   (A âŸ¦ ğ“¸ âŸ§) (Î» i -> âŸ¦ f âŸ§â‚• (args i))
   -- â‰¡âŸ¨ cong ((A âŸ¦_âŸ§)_)
   --    ( âˆ€-extensionality Î» i -> free-unique f g p (args i) ) âŸ©
   --   (A âŸ¦ ğ“¸ âŸ§) (Î» i -> âŸ¦ g âŸ§â‚• (args i))
   -- â‰¡âŸ¨ Eq.sym (Homo g args) âŸ©
   --   âŸ¦ g âŸ§â‚• (node ğ“¸ args)
   -- âˆ

--------------------------
--INTERPRETATION OF TERMS
--------------------------

--(cf Def 4.31 of Bergman)

--Let t âˆˆ Term be a term, A an algebra, in the signature S.
--We define an n-ary operation, denoted (t Ì‚ A), on A by recursion on
--the structure of t, as follows:

-- (1) if t is the variable x âˆˆ X and tup : X -> âŸ¦ A âŸ§áµ¤ is a tuple of elements of A,
--     then we define (t Ì‚ A) tup = tup x.

-- (2) if t = ğ“¸ args, where ğ“¸ âˆˆ âŸ¨ S âŸ©â‚’ is an operation symbol (of arity âŸ¨ S âŸ©â‚ ğ“¸),
--        args : âŸ¨ S âŸ©â‚ ğ“¸ -> Term is an (âŸ¨ S âŸ©â‚ ğ“¸)-tuple of terms, and
--        tup : X -> âŸ¦ A âŸ§áµ¤ is a tuple of elements of A, then we define

--     (t Ì‚ A) tup = ((ğ“¸ args) Ì‚ A) tup
--                  = (A âŸ¦ ğ“¸ âŸ§) Î»{ i -> ((args i) Ì‚ A) tup }

-- Here's the Agda implementation of the foregoing definition.

_Ì‡_ : Term -> (A : algebra S) -> (X -> âŸ¦ A âŸ§áµ¤) -> âŸ¦ A âŸ§áµ¤
((generator x) Ì‡ A) tup = tup x
((node ğ“¸ args) Ì‡ A) tup = (A âŸ¦ ğ“¸ âŸ§) Î»{i -> (args i Ì‡ A) tup }

-- Recall (cf. Theorem 4.32 of Bergman)
--
-- Theorem 1.
-- Let A and B be algebras of type S. Then the following hold:
--
--   (1) For every n-ary term t and homomorphism g: A â€”> B, 
--       g(tá´¬(aâ‚,...,aâ‚™)) = tá´®(g(aâ‚),...,g(aâ‚™)).
--   (2) For every term t âˆˆ T(X) and every Î¸ âˆˆ Con(A), 
--       a Î¸ b => t(a) Î¸ t(b).
--   (3) For every subset Y of A,
--       Sg(Y) = { t(aâ‚,...,aâ‚™) : t âˆˆ T(Xâ‚™), n < Ï‰, and aáµ¢ âˆˆ Y, for i â‰¤ n}.
--
-- PROOF.
--
-- (1) (homomorphisms commute with terms).
comm-hom-term : {A B : algebra S}
  ->    (g : hom A B) -> (t : Term)
  ->    (tup : X -> âŸ¦ A âŸ§áµ¤)
       ------------------------------
  ->     âŸ¦ g âŸ§â‚• ((t Ì‡ A) tup) â‰¡ (t Ì‡ B) (âŸ¦ g âŸ§â‚• âˆ˜ tup)
--
comm-hom-term g (generator x) tup = Eq.refl
comm-hom-term {A} {B} g (node ğ“¸ args) tup =  
-- Goal: âŸ¦ g âŸ§â‚• ((A âŸ¦ ğ“¸ âŸ§) (Î» { i â†’ (args i Ì‡ A) tup })) â‰¡
--       (B âŸ¦ ğ“¸ âŸ§) (Î» { i â†’ (args i Ì‡ B) ((Î» {.x} â†’ âŸ¦ g âŸ§â‚•) âˆ˜ tup) })
  begin
    âŸ¦ g âŸ§â‚• ((A âŸ¦ ğ“¸ âŸ§) (Î» { i â†’ (args i Ì‡ A) tup }))
  â‰¡âŸ¨ homo g ( Î» i â†’ (args i Ì‡ A) tup )âŸ©
    (B âŸ¦ ğ“¸ âŸ§) ( Î» i â†’ âŸ¦ g âŸ§â‚• ((args i Ì‡ A) tup) )
  â‰¡âŸ¨ cong ((B âŸ¦_âŸ§)_)
     ( âˆ€-extensionality  Î» i -> comm-hom-term g (args i) tup  ) âŸ©
    (B âŸ¦ ğ“¸ âŸ§) ( Î» i â†’ (args i Ì‡ B) (âŸ¦ g âŸ§â‚• âˆ˜ tup) )
  âˆ

-- (2) For every term t âˆˆ T(X) and every Î¸ âˆˆ Con(A), 
--     a Î¸ b => t(a) Î¸ t(b).
open con

compatible-term : (A : algebra S)
 ->               (t : Term)
 ->               (Î¸ : con A)
                 -------------------
 ->               compatible-fun (t Ì‡ A) âŸ¦ Î¸ âŸ§áµ£

compatible-term A (generator x) Î¸ p = p x
compatible-term A (node ğ“¸ args) Î¸ p =
  --Goal:
  -- ( âŸ¦ Î¸ âŸ§áµ£ Function.on
  --   ( Î» tup -> (A âŸ¦ ğ“¸ âŸ§) (Î» i -> (args i Ì‡ A) tup) )
  -- ) .i .j
  compat Î¸ ğ“¸ Î»{ i -> (compatible-term A (args i) Î¸) p }

--------------------------------------------------------------
-- analogues for setoid-based algebras

open Setoid

_Ì‚_ : Term -> (A : Algebra S) -> (X -> âˆ¥ âŸ¦ A âŸ§áµ£ âˆ¥) -> âˆ¥ âŸ¦ A âŸ§áµ£ âˆ¥
((generator x) Ì‚ A) tup = tup x
((node ğ“¸ args) Ì‚ A) tup = (A âŸ¦ ğ“¸ âŸ§) Î»{i -> (args i Ì‚ A) tup }

open Con

Compatible-Term :
    (A : Algebra S) -> (t : Term) -> (Î¸ : Con A)
    ----------------------------------------------
  ->   compatible-fun (t Ì‚ A) âŸ¦ Î¸ âŸ§áµ£

Compatible-Term A (generator x) Î¸ p = p x
Compatible-Term A (node ğ“¸ args) Î¸ p =
  compat Î¸  Î»{ k -> (Compatible-Term A (args k) Î¸) p }

--Function.on is the operation,
--  _on_ : âˆ€ {a b c} {A : Set a} {B : Set b} {C : Set c}
--           â†’ (B â†’ B â†’ C) â†’ (A â†’ B) â†’ (A â†’ A â†’ C)
--  _*_ on f = Î» x y â†’ f x * f y
--
--So 
--  (âŸ¦ Î¸ âŸ§áµ£ Function.on (Î» tup â†’ (A âŸ¦ ğ“¸ âŸ§) (Î» { i â†’ (args i Ì‚ A) tup }))) .i .j``
--means
--  ((Î» tup â†’ (A âŸ¦ ğ“¸ âŸ§) (Î» { i â†’ (args i Ì‚ A) tup })) .i)
--  âŸ¦ Î¸ âŸ§áµ£
--  ((Î» tup â†’ (A âŸ¦ ğ“¸ âŸ§) (Î» { i â†’ (args i Ì‚ A) tup })) .j)
--Equivalently,
--   âŸ¦ Î¸ âŸ§áµ£
--    (A âŸ¦ ğ“¸ âŸ§) (Î» { i â†’ (args i Ì‚ A) .i })
--    (A âŸ¦ ğ“¸ âŸ§) (Î» { i â†’ (args i Ì‚ A) .j })                   (1)
--We have,  ``p : lift-rel âŸ¦ Î¸ âŸ§áµ£ .i .j`` and the induction hypothesis,
--    âˆ€ i -> âŸ¦ Î¸ âŸ§áµ£ ((args i Ì‚ A) .i) ((args i Ì‚ A) .j)         (IH)
--which is equivalent to
--    lift-rel âŸ¦ Î¸ âŸ§áµ£ (Î» { i â†’ (args i Ì‚ A) .i }) (Î» { i â†’ (args i Ì‚ A) .j })
--Then we use
--    lift-rel âŸ¦ Î¸ âŸ§áµ£ =[ (A âŸ¦ ğ“¸ âŸ§) ]â‡’ âŸ¦ Î¸ âŸ§áµ£                    (2)
--to get (1).
--We get (2) from: compatible-alg A âŸ¦ Î¸ âŸ§áµ£ {ğ“¸}, which we get from ``compat Î¸ {ğ“¸}``
--We get (IH) from: 
--
--  induct : (A : algebra S)
--    ->     (Î¸ : con A)
--    ->     (args : â„• â†’ Term)
--    ->     (i : Fin (âŸ¨ S âŸ©â‚ ğ“¸))
--          -------------------
--    ->     compatible-fun (args i Ì‚ A) âŸ¦ Î¸ âŸ§áµ£
--  induct A Î¸ args i = compatible-term A (args i) Î¸ 

---------------------------------------------------------

-- ARITY OF A TERM
argsum : â„• -> (â„• -> â„•) -> â„•
argsum nzero f = 0
argsum (succ n) f = f n + argsum n f

âŸ¨_âŸ©â‚œ : Term -> â„•
âŸ¨ generator x âŸ©â‚œ = 1
âŸ¨ node ğ“¸ args âŸ©â‚œ = (S Ï) ğ“¸ + argsum ((S Ï) ğ“¸) (Î» i -> âŸ¨ args i âŸ©â‚œ)


-------------------------------------------------------------


--Alternative approach to interpretation.

-- Essential arity
------------------

-- The definition of "arity" of a term is a bit nuanced as the following example shows:

-- Example. Suppose ğ‘“ is a binary term, and ğ‘ and ğ‘ are ternary terms.

-- How should we define the "arity" of the following term?

--   ğ‘“(ğ‘(ğ‘¥, ğ‘¦, ğ‘§), f(ğ‘¤, ğ‘¥), ğ‘(ğ‘¢, ğ‘£, ğ‘¤))

-- On the face of it, it seems safe to say t has arity 6 since we express it as a function
-- of 6 variables as follows:

--   t(ğ‘¢, ğ‘£, ğ‘¤, ğ‘¥, ğ‘¦, ğ‘§) = ğ‘“(ğ‘(ğ‘¥, ğ‘¦, ğ‘§), ğ‘“(ğ‘¤, ğ‘¥), ğ‘(ğ‘¢, ğ‘£, ğ‘¤))

-- But what if ğ‘(ğ‘¥,ğ‘¦,ğ‘§) = ğ‘§?  Then we would say that the "essential arity" of g is 1 since
-- we can express g and t equivalently as ğ‘'(ğ‘§) = ğ‘(ğ‘¥,ğ‘¦,ğ‘§) and 

--   t'(ğ‘¢, ğ‘£, ğ‘¤, ğ‘¥, ğ‘§) = ğ‘“(ğ‘'(ğ‘§), ğ‘“(ğ‘¤, ğ‘¥), ğ‘(ğ‘¢, ğ‘£, ğ‘¤)),

-- resp., in which case it seems the "arity" of t is really 5 (or maybe, to be safe, *at most* 5).

-- By now it should be clear that we can't know the *essential* arity of t (that is, the minimum
-- number of variables required to express t) until we know the essential arities of ğ‘“, ğ‘, and ğ‘.

-- If, for example, ğ‘(ğ‘¢, ğ‘£, ğ‘¤) = ğ‘“(ğ‘£, ğ‘¤), then t is expressible as

--  t''(ğ‘£, ğ‘¤, ğ‘¥, ğ‘§) = ğ‘“(ğ‘'(ğ‘§), ğ‘“(ğ‘¤, ğ‘¥), ğ‘“(ğ‘£, ğ‘¤))

-- If moreover we know that ğ‘“ has essential arity 2, then this is as far as we can reduce the
-- argument list of t so we can conclude that t has essential arity 4.


--Interpretation of Terms
--========================

-- Now, if X = {xâ‚€, xâ‚, xâ‚‚,...}, then we can re-write the term in the following equivalent way:

--   t(xâ‚€, xâ‚, xâ‚‚, xâ‚ƒ, xâ‚„, xâ‚…) = f(g(xâ‚ƒ, xâ‚„, xâ‚…), f(xâ‚‚, xâ‚ƒ), h(xâ‚€, xâ‚, xâ‚‚)).

-- If ğ’™ : Ï‰ -> X, where ğ’™ ğ‘– = xáµ¢, then t can be expressed as

--   t ğ’™ = f(g(Ï€â‚ƒğ’™, Ï€â‚„ğ’™, Ï€â‚…ğ’™), f(Ï€â‚‚ğ’™, Ï€â‚ƒğ’™), h(Ï€â‚€ğ’™, Ï€â‚ğ’™, Ï€â‚‚ğ’™)),

-- where Ï€áµ¢ is the project onto the (zero offset) ğ‘–-th coordinate.

-- (N.B. "zero offset" means that the smallest index (subscript) is 0; to avoid confusion, we refer to this as the index not of the "1st coordinate" but of the "0th coordinate.")
--Given a set ``X`` and an algebra ``ğ€ = âŸ¨A,...âŸ©``, we call a function ``ctx : X â†’ A`` a **context**.

--**Definition**. (cf Def 4.31 of Bergman)
--
--Let :math:`t` be a term of arity :math:`Ï t`, and ğ€ an algebra, in the signature :math:`S`.
--
--The **interpretation** of :math:`t` in ğ€---often denoted in the literature by :math:`t^ğš¨`---is the :math:`(Ï t)`-ary operation on :math:`A` defined by recursion on the structure of :math:`t`, as follows:

--1. if :math:`t` is the variable :math:`x âˆˆ X`, then in the context ``ctx`` we take :math:`t^ğš¨` to be the projection onto the coordinate containing ``ctx x``.

--2. if :math:`t = ğ“¸ ğŸ`, where ğ“¸ is a basic operation symbol with interpretation :math:`ğ“¸^ğš¨` in ğš¨ and :math:`ğŸ : (Ï ğ“¸) â†’` Term is a (Ï ğ“¸)-tuple of terms, each with interpretation :math:`(ğŸ i)^ğš¨`, then we take :math:`t^ğ€(ğŸ)` to be :math:`ğ“¸^ğ€ \bigl( Î» \{ (i : Ï ğ“¸) . (ğŸ i)^ğ€\}\bigr)`.

-- Let's translate this definition using the Agda syntax we developed above.

-- Let ``t`` be a term, ğ€ an algebra,  of signature ``S``.

-- The **interpretation** of :math:`t` in ğ€---often denoted in the literature by :math:`t^ğš¨`---is an operation of :math:`A` defined by recursion on the structure of :math:`t`.

-- 1. If ``t`` is a variable, say, ``x : X``, then we define ``(t Ì‚ A) : âŸ¦ A âŸ§áµ¤ -> âŸ¦ A âŸ§áµ¤`` for each ``a : âŸ¦ A âŸ§áµ¤`` by ``(t Ì‚ A) a = a``.
-- 2. If ``t = ğ“¸ ğŸ``, where ``ğ“¸ : âŸ¨ S âŸ©â‚’`` is a basic operation symbol with interpretation ``A âŸ¦ ğ“¸ âŸ§`` in ğš¨, and if ``ğŸ : âŸ¨ S âŸ©â‚ ğ“¸ -> Term`` is a ``(âŸ¨ S âŸ©â‚ ğ“¸)``-tuple of terms with interpretations ``(ğŸ i) Ì‚ A`` for each ``i : âŸ¨ S âŸ©â‚ ğ“¸``, then we define
--    ``(t Ì‚ A) = (ğ“¸ ğŸ) Ì‚ A = (A âŸ¦ ğ“¸ âŸ§) Î»{i -> (ğŸ i) Ì‚ A}``

-- Here's how we would implement this in Agda.
-- .. code-block:: agda
--    _Ì‚_ : {â„“â‚ : Level} -> Term -> (A : algebra {â„“â‚} S) -> (X -> âŸ¦ A âŸ§áµ¤) -> âŸ¦ A âŸ§áµ¤
--    ((generator x) Ì‚ A) tup = tup x
--    ((node ğ“¸ args) Ì‚ A) tup = (A âŸ¦ ğ“¸ âŸ§) Î»{i -> (args i Ì‚ A) tup }


