--File: free.agda
--Author: William DeMeo
--Date: 25 Dec 2019
--Updated: 10 Jan 2020
--Note: This was used for the second part of my talk at JMM Special Session.

{-# OPTIONS --without-K --exact-split #-}

open import Level
open import basic 
open signature

module free {S : signature}{X : Set} where

open import preliminaries  using (_âŠ_ ; âˆ€-extensionality; âˆ‘)
open import Function using (_âˆ˜_)
open import Relation.Unary
open import Relation.Binary hiding (Total)
import Relation.Binary.PropositionalEquality as Eq
open Eq using (_â‰¡_; refl; cong; sym; isEquivalence)
open Eq.â‰¡-Reasoning
import Relation.Binary.EqReasoning as EqR

--------------------------------------------------------------

----------------------------
-- TERMS in the signature S
----------------------------

data Term : Set where
  generator : X -> Term
  node : âˆ€ (ğ“¸ : âŸ¨ S âŸ©â‚’) -> (Fin (âŸ¨ S âŸ©â‚ ğ“¸) -> Term) -> Term


----------------------------------
-- TERM ALGEBRA (for signature S)
----------------------------------

open algebra
open Term


free : algebra S

free = record { âŸ¦_âŸ§áµ¤ = Term ; _âŸ¦_âŸ§ = node }

--------------------------------------------------------------
-- analogue for setoid-based algebras

open Algebra

Free : Algebra S
Free = record {
         âŸ¦_âŸ§áµ£ = record {
                 Carrier = Term ;
                 _â‰ˆ_ = _â‰¡_ ;
                 isEquivalence = isEquivalence
                 } ;
         _âŸ¦_âŸ§ = node  }

-------------------------------------
-- The UNIVERSAL PROPERTY of free
-- 1. every h : X -> âŸ¦ A âŸ§áµ¤  lifts to a hom from free to A.
-- 2. the induced hom is unique.

-- PROOF.
-- 1.a. Every map  (X -> A)  "lifts".
free-lift : {A : algebra  S}(h : X -> âŸ¦ A âŸ§áµ¤) -> âŸ¦ free âŸ§áµ¤ -> âŸ¦ A âŸ§áµ¤
free-lift h (generator x) = h x
free-lift {A} h (node ğ“¸ args) = (A âŸ¦ ğ“¸ âŸ§) Î»{i -> free-lift {A} h (args i)}
-- 1.b. The lift is a hom.
open hom
lift-hom : {A : algebra S} (h : X -> âŸ¦ A âŸ§áµ¤) -> hom free A
lift-hom {A} h = record { âŸ¦_âŸ§â‚• = free-lift {A} h; homo = Î» args â†’ refl }

-- 2. The lift to  (free -> A)  is unique.
--    (We need EXTENSIONALITY for this (imported from util.agda))
free-unique : {A : algebra S}
  ->    ( f g : hom free A )
  ->    ( âˆ€ x  ->  âŸ¦ f âŸ§â‚• (generator x) â‰¡ âŸ¦ g âŸ§â‚• (generator x) )
  ->    (t : Term)
       ---------------------------
  ->    âŸ¦ f âŸ§â‚• t â‰¡ âŸ¦ g âŸ§â‚• t

free-unique {A} f g p (generator x) = p x
free-unique {A} f g p (node ğ“¸ args) =
   begin
     âŸ¦ f âŸ§â‚• (node ğ“¸ args)
   â‰¡âŸ¨ homo f args  âŸ©
     (A âŸ¦ ğ“¸ âŸ§) (Î» i -> âŸ¦ f âŸ§â‚• (args i))
   â‰¡âŸ¨ cong ((A âŸ¦_âŸ§)_)
      ( âˆ€-extensionality Î» i -> free-unique f g p (args i) ) âŸ©
     (A âŸ¦ ğ“¸ âŸ§) (Î» i -> âŸ¦ g âŸ§â‚• (args i))
   â‰¡âŸ¨ sym (homo g args) âŸ©
     âŸ¦ g âŸ§â‚• (node ğ“¸ args)
   âˆ

----------------------------------------
-- setoid-based analogues

open Setoid 
Free-Lift : {A : Algebra  S}(h : X -> Carrier âŸ¦ A âŸ§áµ£) -> Carrier âŸ¦ Free âŸ§áµ£ -> Carrier âŸ¦ A âŸ§áµ£
Free-Lift h (generator x) = h x
Free-Lift {A} h (node ğ“¸ args) = (A âŸ¦ ğ“¸ âŸ§) Î» i -> Free-Lift {A} h (args i)

----------------------------------------

-- 1.b. The lift is a hom.

open Hom

Lift-Hom : {A : Algebra S} (h : X -> Carrier âŸ¦ A âŸ§áµ£) -> Hom Free A
Lift-Hom {A} h = record { âŸ¦_âŸ§â‚• = Free-Lift {A} h; Homo = Î» args â†’ Setoid.refl âŸ¦ A âŸ§áµ£ }



--------------------------
--INTERPRETATION OF TERMS
--------------------------

--(cf Def 4.31 of Bergman)

--Let t âˆˆ Term be a term, A an algebra, in the signature S.
--We define an n-ary operation, denoted (t Ì‚ A), on A by recursion on
--the structure of t, as follows:

-- (1) if t is the variable x âˆˆ X and tup : X -> âŸ¦ A âŸ§áµ¤ is a tuple of elements of A,
--     then we define (t Ì‚ A) tup = tup x.

-- (2) if t = ğ“¸ args, where ğ“¸ âˆˆ âŸ¨ S âŸ©â‚’ is an operation symbol (of arity âŸ¨ S âŸ©â‚ ğ“¸),
--        args : âŸ¨ S âŸ©â‚ ğ“¸ -> Term is an (âŸ¨ S âŸ©â‚ ğ“¸)-tuple of terms, and
--        tup : X -> âŸ¦ A âŸ§áµ¤ is a tuple of elements of A, then we define

--     (t Ì‚ A) tup = ((ğ“¸ args) Ì‚ A) tup
--                  = (A âŸ¦ ğ“¸ âŸ§) Î»{ i -> ((args i) Ì‚ A) tup }


-- Here's the Agda implementation of the foregoing definition.

_Ì‡_ : Term -> (A : algebra S) -> (X -> âŸ¦ A âŸ§áµ¤) -> âŸ¦ A âŸ§áµ¤
((generator x) Ì‡ A) tup = tup x
((node ğ“¸ args) Ì‡ A) tup = (A âŸ¦ ğ“¸ âŸ§) Î»{i -> (args i Ì‡ A) tup }

-- Recall, Theorem 4.32 of Bergman.
-- Let A and B be algebras of type S. Then the following hold:
--
--   (1) For every n-ary term t and homomorphism g: A â€”> B, 
--       g(tá´¬(aâ‚,...,aâ‚™)) = tá´®(g(aâ‚),...,g(aâ‚™)).
--   (2) For every term t âˆˆ T(X) and every Î¸ âˆˆ Con(A), 
--       a Î¸ b => t(a) Î¸ t(b).
--   (3) For every subset Y of A,
--       Sg(Y) = { t(aâ‚,...,aâ‚™) : t âˆˆ T(Xâ‚™), n < Ï‰, and aáµ¢ âˆˆ Y, for i â‰¤ n}.
--
-- PROOF of (1)
--
-- (1) homomorphisms commute with terms
--
comm-hom-term : {A B : algebra S}
  ->    (g : hom A B) -> (t : Term)
  ->    (tup : X -> âŸ¦ A âŸ§áµ¤)
       ------------------------------
  ->     âŸ¦ g âŸ§â‚• ((t Ì‡ A) tup) â‰¡ (t Ì‡ B) (âŸ¦ g âŸ§â‚• âˆ˜ tup)
--
comm-hom-term g (generator x) tup = Eq.refl
comm-hom-term {A} {B} g (node ğ“¸ args) tup =  
-- Goal: âŸ¦ g âŸ§â‚• ((A âŸ¦ ğ“¸ âŸ§) (Î» { i â†’ (args i Ì‡ A) tup })) â‰¡
--       (B âŸ¦ ğ“¸ âŸ§) (Î» { i â†’ (args i Ì‡ B) ((Î» {.x} â†’ âŸ¦ g âŸ§â‚•) âˆ˜ tup) })
  begin
    âŸ¦ g âŸ§â‚• ((A âŸ¦ ğ“¸ âŸ§) (Î» { i â†’ (args i Ì‡ A) tup }))
  â‰¡âŸ¨ homo g ( Î» i â†’ (args i Ì‡ A) tup )âŸ©
    (B âŸ¦ ğ“¸ âŸ§) ( Î» i â†’ âŸ¦ g âŸ§â‚• ((args i Ì‡ A) tup) )
  â‰¡âŸ¨ cong ((B âŸ¦_âŸ§)_)
     ( âˆ€-extensionality  Î» i -> comm-hom-term g (args i) tup  ) âŸ©
    (B âŸ¦ ğ“¸ âŸ§) ( Î» i â†’ (args i Ì‡ B) (âŸ¦ g âŸ§â‚• âˆ˜ tup) )
  âˆ

--
--
-- PROOF of (2).
--
-- (2) For every term t âˆˆ T(X) and every Î¸ âˆˆ Con(A), 
--     a Î¸ b => t(a) Î¸ t(b).
--
open con

compatible-term : (A : algebra S)
 ->               (t : Term)
 ->               (Î¸ : con A)
                 -------------------
 ->               compatible-fun (t Ì‡ A) âŸ¦ Î¸ âŸ§áµ£

compatible-term A (generator x) Î¸ p = p x
compatible-term A (node ğ“¸ args) Î¸ p =
  --Goal:
  -- ( âŸ¦ Î¸ âŸ§áµ£ Function.on
  --   ( Î» tup -> (A âŸ¦ ğ“¸ âŸ§) (Î» i -> (args i Ì‡ A) tup) )
  -- ) .i .j
  compat Î¸ ğ“¸ Î»{ i -> (compatible-term A (args i) Î¸) p }

--------------------------------------------------------------
-- analogues for setoid-based algebras

open Setoid

_Ì‚_ : Term -> (A : Algebra S) -> (X -> Carrier âŸ¦ A âŸ§áµ£) -> Carrier âŸ¦ A âŸ§áµ£
((generator x) Ì‚ A) tup = tup x
((node ğ“¸ args) Ì‚ A) tup = (A âŸ¦ ğ“¸ âŸ§) Î»{i -> (args i Ì‚ A) tup }

open Con

Compatible-Term :
    (A : Algebra S) -> (t : Term) -> (Î¸ : Con A)
    ----------------------------------------------
  ->   compatible-fun (t Ì‚ A) âŸ¦ Î¸ âŸ§áµ£

Compatible-Term A (generator x) Î¸ p = p x
Compatible-Term A (node ğ“¸ args) Î¸ p =
  compat Î¸  Î»{ k -> (Compatible-Term A (args k) Î¸) p }

--Function.on is the operation,
--  _on_ : âˆ€ {a b c} {A : Set a} {B : Set b} {C : Set c}
--           â†’ (B â†’ B â†’ C) â†’ (A â†’ B) â†’ (A â†’ A â†’ C)
--  _*_ on f = Î» x y â†’ f x * f y
--
--So 
--  (âŸ¦ Î¸ âŸ§áµ£ Function.on (Î» tup â†’ (A âŸ¦ ğ“¸ âŸ§) (Î» { i â†’ (args i Ì‚ A) tup }))) .i .j``
--means
--  ((Î» tup â†’ (A âŸ¦ ğ“¸ âŸ§) (Î» { i â†’ (args i Ì‚ A) tup })) .i)
--  âŸ¦ Î¸ âŸ§áµ£
--  ((Î» tup â†’ (A âŸ¦ ğ“¸ âŸ§) (Î» { i â†’ (args i Ì‚ A) tup })) .j)
--Equivalently,
--   âŸ¦ Î¸ âŸ§áµ£
--    (A âŸ¦ ğ“¸ âŸ§) (Î» { i â†’ (args i Ì‚ A) .i })
--    (A âŸ¦ ğ“¸ âŸ§) (Î» { i â†’ (args i Ì‚ A) .j })                   (1)
--We have,  ``p : lift-rel âŸ¦ Î¸ âŸ§áµ£ .i .j`` and the induction hypothesis,
--    âˆ€ i -> âŸ¦ Î¸ âŸ§áµ£ ((args i Ì‚ A) .i) ((args i Ì‚ A) .j)         (IH)
--which is equivalent to
--    lift-rel âŸ¦ Î¸ âŸ§áµ£ (Î» { i â†’ (args i Ì‚ A) .i }) (Î» { i â†’ (args i Ì‚ A) .j })
--Then we use
--    lift-rel âŸ¦ Î¸ âŸ§áµ£ =[ (A âŸ¦ ğ“¸ âŸ§) ]â‡’ âŸ¦ Î¸ âŸ§áµ£                    (2)
--to get (1).
--We get (2) from: compatible-alg A âŸ¦ Î¸ âŸ§áµ£ {ğ“¸}, which we get from ``compat Î¸ {ğ“¸}``
--We get (IH) from: 
--
--  induct : (A : algebra S)
--    ->     (Î¸ : con A)
--    ->     (args : Fin (âŸ¨ S âŸ©â‚ ğ“¸) â†’ Term)
--    ->     (i : Fin (âŸ¨ S âŸ©â‚ ğ“¸))
--          -------------------
--    ->     compatible-fun (args i Ì‚ A) âŸ¦ Î¸ âŸ§áµ£
--  induct A Î¸ args i = compatible-term A (args i) Î¸ 


-----------------------------


--After inserting `` (compat Î¸ ğ“¸) ?``, the  new goal is:
-- Goal: lift-rel âŸ¦ Î¸ âŸ§áµ£ (Î» { i â†’ (args i Ì‚ A) .i })
--       (Î» { i â†’ (args i Ì‚ A) .j })
-- â€”â€”â€”â€”â€”â€”â€”â€”â€”â€”â€”â€”â€”â€”â€”â€”â€”â€”â€”â€”â€”â€”â€”â€”â€”â€”â€”â€”â€”â€”â€”â€”â€”â€”â€”â€”â€”â€”â€”â€”â€”â€”â€”â€”â€”â€”â€”â€”â€”â€”â€”â€”â€”â€”â€”â€”â€”â€”â€”â€”
-- p    : lift-rel âŸ¦ Î¸ âŸ§áµ£ .i .j
-- .j   : X â†’ âŸ¦ A âŸ§áµ¤
-- .i   : X â†’ âŸ¦ A âŸ§áµ¤
-- Î¸    : con A
-- args : Fin (âŸ¨ S âŸ©â‚ ğ“¸) â†’ Term
-- ğ“¸    : âŸ¨ S âŸ©â‚’
-- A    : algebra S
-- X    : Set
-- S    : signature

--------------------------------------------------
