--File: Free.agda
--Author: William DeMeo and Siva Somayyajula
--Date: 20 Feb 2020
--Updated: 21 Feb 2020
--Notes: Based on the file `free.agda` (25 Dec 2019).
--       Used for 2nd half of talk at JMM Special Session (Jan 2020).

{-# OPTIONS --without-K --exact-split #-}

open import Preliminaries
open import Basic 
open import Hom
open import Con

module Free {i j k : Level} {S : Signature i j} {X : Set k}  where

----------------------------
-- TERMS in the signature S
----------------------------
-- open signature

data Term : Set (i âŠ” j âŠ” k) where
  generator : X -> Term
  node : (ğ“¸ : âˆ£ S âˆ£) -> (ğ’• : âŸ¦ S âŸ§ ğ“¸ -> Term) -> Term

open Term

map-Term : (Term -> Term) -> Term -> Term
map-Term f (generator x) = f (generator x)
map-Term f (node ğ“¸ ğ’•) = node ğ“¸ (Î» i -> map-Term f (ğ’• i))

----------------------------------
-- TERM ALGEBRA (for signature S)
----------------------------------

-- open Algebra
-- open Term

ğ”‰ : Algebra (i âŠ” j âŠ” k) S
ğ”‰ = Term , node
--record { âŸ¦_âŸ§áµ¤ = Term ; _âŸ¦_âŸ§ = node }
-------------------------------------
-- The UNIVERSAL PROPERTY of free

-- We first prove this for algebras whose carriers are mere sets.

-- 1. every h : X -> âŸ¦ A âŸ§áµ¤  lifts to a hom from free to A.
-- 2. the induced hom is unique.

-- PROOF.
-- 1.a. Every map  (X -> A)  "lifts".
--âˆ€{â„“ : Level} 
--free-lift : {ğ‘¨ : Algebra  (i âŠ” j âŠ” k) S}
free-lift : {ğ‘¨ : Algebra  k S}
  ->        (h : X -> âˆ£ ğ‘¨ âˆ£)
          -----------------------------------
  ->        âˆ£ ğ”‰ âˆ£ -> âˆ£ ğ‘¨ âˆ£
free-lift h (generator x) = h x
free-lift {ğ‘¨} h (node ğ“¸ args) =
  (âŸ¦ ğ‘¨ âŸ§ ğ“¸) Î»{i -> free-lift {ğ‘¨} h (args i)}

-- 1.b. The lift is a hom.
--lift-hom : {ğ‘¨ : Algebra (i âŠ” j âŠ” k) S}
lift-hom : {ğ‘¨ : Algebra k S}
  ->       (h : X -> âˆ£ ğ‘¨ âˆ£)
          ------------------------------------
  ->       Hom ğ”‰ ğ‘¨
lift-hom {ğ‘¨} h = free-lift {ğ‘¨} h , Î» ğ“¸ ğ’‚ â†’ cong (âŸ¦ ğ‘¨ âŸ§ _) refl
--record { âŸ¦_âŸ§â‚• = free-lift {A} h; homo = Î» args â†’ refl }

-- 2. The lift to  (free -> A)  is unique.
--    (We need EXTENSIONALITY for this (imported from util.agda))
free-unique : {ğ‘¨ : Algebra k S}
  ->    ( f g : Hom ğ”‰ ğ‘¨ )
  ->    ( âˆ€ x  ->  âˆ£ f âˆ£ (generator x) â‰¡ âˆ£ g âˆ£ (generator x) )
  ->    (t : Term)
       ---------------------------
  ->    âˆ£ f âˆ£ t â‰¡ âˆ£ g âˆ£ t

free-unique f g p (generator x) = p x
free-unique {ğ‘¨} f g p (node ğ“¸ args) =
   begin
     ( âˆ£ f âˆ£ )(node ğ“¸ args)
   â‰¡âŸ¨ âŸ¦ f âŸ§ ğ“¸ args âŸ©
     (âŸ¦ ğ‘¨ âŸ§ ğ“¸) (Î» i -> âˆ£ f âˆ£ (args i))
   â‰¡âŸ¨ cong (âŸ¦ ğ‘¨ âŸ§ _)
        (âˆ€-extensionality-â„“â‚-â„“â‚‚ {j} {k}
          ( Î» i -> free-unique {ğ‘¨} f g p (args i))
        )
    âŸ©
     (âŸ¦ ğ‘¨ âŸ§ ğ“¸) (Î» i -> âˆ£ g âˆ£ (args i))
   â‰¡âŸ¨ sym (âŸ¦ g âŸ§ ğ“¸ args) âŸ©
     âˆ£ g âˆ£ (node ğ“¸ args)
   âˆ

--------------------------
--INTERPRETATION OF TERMS
--------------------------
--(cf Def 4.31 of Bergman)
--Let ğ’• : Term be a term, ğ‘¨ an algebra, in the signature S. We define an
--n-ary operation, denoted (ğ’• Ì‚ ğ‘¨), on ğ‘¨ by recursion on the struct of ğ’•.
-- 1. if ğ’• is the var x âˆˆ X, ğ’‚ : X -> âˆ£ ğ‘¨ âˆ£ a tuple from A, then (t Ì‚ ğ‘¨) ğ’‚ = ğ’‚ x.
-- 2. if ğ’• = ğ“¸ args, ğ“¸ âˆˆ âˆ£ S âˆ£ an op symbol, args : âŸ¦ S âŸ§ ğ“¸ -> Term a
--    (âŸ¦ S âŸ§ ğ“¸)-tuple of terms, ğ’‚ : X -> âˆ£ A âˆ£ a tuple from A, then
--    (t Ì‚ ğ‘¨) ğ’‚ = ((ğ“¸ args) Ì‚ ğ‘¨) ğ’‚ = (âŸ¦ ğ‘¨ âŸ§ ğ“¸) Î»{ i -> ((args i) Ì‚ ğ‘¨) ğ’‚ }
-- module _ {Sâ‚ : Signature (lsuc i) (lsuc j)} {ğ‘¨ ğ‘© : Algebra (i âŠ” j âŠ” â„“) Sâ‚} where

-- _Ì‡_ : Term -> (ğ‘¨ : Algebra (i âŠ” j âŠ” k) S) -> (X -> âˆ£ ğ‘¨ âˆ£) -> âˆ£ ğ‘¨ âˆ£
_Ì‡_ : Term -> (ğ‘¨ : Algebra k S) -> (X -> âˆ£ ğ‘¨ âˆ£) -> âˆ£ ğ‘¨ âˆ£
((generator x) Ì‡ ğ‘¨) ğ’‚ = ğ’‚ x
((node ğ“¸ args) Ì‡ ğ‘¨) ğ’‚ = (âŸ¦ ğ‘¨ âŸ§ ğ“¸) Î»{i -> ((args i) Ì‡ ğ‘¨) ğ’‚ }-- (_Ì‡_ {ğ‘¨} (args i) ğ‘¨) ğ’‚ }

  -- Recall (cf. Theorem 4.32 of Bergman)
  -- Theorem 1.
  -- Let A and B be algebras of type S. Then the following hold:
  -- 1. For every n-ary term t and homomorphism g: A â€”> B, 
  --    g(tá´¬(aâ‚,...,aâ‚™)) = tá´®(g(aâ‚),...,g(aâ‚™)).
  -- 2. For every term t âˆˆ T(X) and every Î¸ âˆˆ Con(A), 
  --    a Î¸ b => t(a) Î¸ t(b).
  -- 3. For every subset Y of A,
  --    Sg(Y) = {t(aâ‚,...,aâ‚™) : t âˆˆ T(Xâ‚™), n < Ï‰, aáµ¢ âˆˆ Y, i â‰¤ n}.
  -- PROOF.
  -- 1. (homomorphisms commute with terms).
comm-hom-term : (ğ‘¨ ğ‘© : Algebra k S)
  ->            (g : Hom ğ‘¨ ğ‘©) -> (ğ’• : Term)   -- {ğ‘¨ ğ‘© : Algebra (i âŠ” j âŠ” â„“) S}
  ->            (ğ’‚ : X -> âˆ£ ğ‘¨ âˆ£)
              ----------------------------------------
  ->            âˆ£ g âˆ£ ((ğ’• Ì‡ ğ‘¨) ğ’‚) â‰¡ (ğ’• Ì‡ ğ‘©) (âˆ£ g âˆ£ âˆ˜ ğ’‚)

comm-hom-term ğ‘¨ ğ‘© g (generator x) ğ’‚ = refl
comm-hom-term ğ‘¨ ğ‘© g (node ğ“¸ args) ğ’‚ =
  begin
    âˆ£ g âˆ£ (âŸ¦ ğ‘¨ âŸ§ ğ“¸ (Î» iâ‚ â†’ (args iâ‚ Ì‡ ğ‘¨) ğ’‚))
  â‰¡âŸ¨ âŸ¦ g âŸ§ ğ“¸ ( Î» r â†’ (args r Ì‡ ğ‘¨) ğ’‚ ) âŸ©
    (âŸ¦ ğ‘© âŸ§ ğ“¸) ( Î» iâ‚ â†’  âˆ£ g âˆ£ ((args iâ‚ Ì‡ ğ‘¨) ğ’‚) )
    â‰¡âŸ¨ cong (âŸ¦ ğ‘© âŸ§ _) (( âˆ€-extensionality-â„“â‚-â„“â‚‚ {j} {k}
                         (Î» iâ‚ -> comm-hom-term ğ‘¨ ğ‘© g (args iâ‚) ğ’‚  )
                      ))
     âŸ©
    (âŸ¦ ğ‘© âŸ§ ğ“¸) ( Î» r -> (args r Ì‡ ğ‘©) (âˆ£ g âˆ£ âˆ˜ ğ’‚) )
  âˆ

  --For 2 of Thm 1, we need congruences (see Congruence.agda).
  -- 2. If t : Term, Î¸ : Con A, then a Î¸ b => t(a) Î¸ t(b).
compatible-term : (ğ‘¨ : Algebra k S)
  ->              (ğ’• : Term)
  ->              (Î¸ : Con ğ‘¨)
                 ------------------------------------
  ->              compatible-fun {i} {j} {k} {S} (ğ’• Ì‡ ğ‘¨) âˆ£ Î¸ âˆ£
  -- wjd: I don't know why this ^^^^^^^^^^^^^^^^^ combination
  --      of implicit vars works... very weird.

compatible-term ğ‘¨ (generator x) Î¸ p = p x
compatible-term ğ‘¨ (node ğ“¸ args) Î¸ p =
  âŸ¦ âŸ¦ Î¸ âŸ§ âŸ§ ğ“¸ Î»{ x -> (compatible-term ğ‘¨ (args x) Î¸) p }

---------------------------------------------------------

-- ARITY OF A TERM
-- argsum : â„• -> (â„• -> â„•) -> â„•
-- argsum nzero f = 0
-- argsum (succ n) f = f n + argsum n f

-- âŸ¨_âŸ©â‚œ : Term -> â„•
-- âŸ¨ generator x âŸ©â‚œ = 1
-- âŸ¨ node ğ“¸ args âŸ©â‚œ = (S Ï) ğ“¸ + argsum ((S Ï) ğ“¸) (Î» i -> âŸ¨ args i âŸ©â‚œ)


-------------------------------------------------------------


--Alternative approach to interpretation.

-- Essential arity
------------------

-- The definition of "arity" of a term is a bit nuanced as the following example shows:

-- Example. Suppose ğ‘“ is a binary term, and ğ‘ and ğ‘ are ternary terms.

-- How should we define the "arity" of the following term?

--   ğ‘“(ğ‘(ğ‘¥, ğ‘¦, ğ‘§), f(ğ‘¤, ğ‘¥), ğ‘(ğ‘¢, ğ‘£, ğ‘¤))

-- On the face of it, it seems safe to say t has arity 6 since we express it as a function
-- of 6 variables as follows:

--   t(ğ‘¢, ğ‘£, ğ‘¤, ğ‘¥, ğ‘¦, ğ‘§) = ğ‘“(ğ‘(ğ‘¥, ğ‘¦, ğ‘§), ğ‘“(ğ‘¤, ğ‘¥), ğ‘(ğ‘¢, ğ‘£, ğ‘¤))

-- But what if ğ‘(ğ‘¥,ğ‘¦,ğ‘§) = ğ‘§?  Then we would say that the "essential arity" of g is 1 since
-- we can express g and t equivalently as ğ‘'(ğ‘§) = ğ‘(ğ‘¥,ğ‘¦,ğ‘§) and 

--   t'(ğ‘¢, ğ‘£, ğ‘¤, ğ‘¥, ğ‘§) = ğ‘“(ğ‘'(ğ‘§), ğ‘“(ğ‘¤, ğ‘¥), ğ‘(ğ‘¢, ğ‘£, ğ‘¤)),

-- resp., in which case it seems the "arity" of t is really 5 (or maybe, to be safe, *at most* 5).

-- By now it should be clear that we can't know the *essential* arity of t (that is, the minimum
-- number of variables required to express t) until we know the essential arities of ğ‘“, ğ‘, and ğ‘.

-- If, for example, ğ‘(ğ‘¢, ğ‘£, ğ‘¤) = ğ‘“(ğ‘£, ğ‘¤), then t is expressible as

--  t''(ğ‘£, ğ‘¤, ğ‘¥, ğ‘§) = ğ‘“(ğ‘'(ğ‘§), ğ‘“(ğ‘¤, ğ‘¥), ğ‘“(ğ‘£, ğ‘¤))

-- If moreover we know that ğ‘“ has essential arity 2, then this is as far as we can reduce the
-- argument list of t so we can conclude that t has essential arity 4.


--Interpretation of Terms
--========================

-- Now, if X = {xâ‚€, xâ‚, xâ‚‚,...}, then we can re-write the term in the following equivalent way:

--   t(xâ‚€, xâ‚, xâ‚‚, xâ‚ƒ, xâ‚„, xâ‚…) = f(g(xâ‚ƒ, xâ‚„, xâ‚…), f(xâ‚‚, xâ‚ƒ), h(xâ‚€, xâ‚, xâ‚‚)).

-- If ğ’™ : Ï‰ -> X, where ğ’™ ğ‘– = xáµ¢, then t can be expressed as

--   t ğ’™ = f(g(Ï€â‚ƒğ’™, Ï€â‚„ğ’™, Ï€â‚…ğ’™), f(Ï€â‚‚ğ’™, Ï€â‚ƒğ’™), h(Ï€â‚€ğ’™, Ï€â‚ğ’™, Ï€â‚‚ğ’™)),

-- where Ï€áµ¢ is the project onto the (zero offset) ğ‘–-th coordinate.

-- (N.B. "zero offset" means that the smallest index (subscript) is 0; to avoid confusion, we refer to this as the index not of the "1st coordinate" but of the "0th coordinate.")
--Given a set ``X`` and an algebra ``ğ€ = âŸ¨A,...âŸ©``, we call a function ``ctx : X â†’ A`` a **context**.

--**Definition**. (cf Def 4.31 of Bergman)
--
--Let :math:`t` be a term of arity :math:`Ï t`, and ğ€ an algebra, in the signature :math:`S`.
--
--The **interpretation** of :math:`t` in ğ€---often denoted in the literature by :math:`t^ğš¨`---is the :math:`(Ï t)`-ary operation on :math:`A` defined by recursion on the structure of :math:`t`, as follows:

--1. if :math:`t` is the variable :math:`x âˆˆ X`, then in the context ``ctx`` we take :math:`t^ğš¨` to be the projection onto the coordinate containing ``ctx x``.

--2. if :math:`t = ğ“¸ ğŸ`, where ğ“¸ is a basic operation symbol with interpretation :math:`ğ“¸^ğš¨` in ğš¨ and :math:`ğŸ : (Ï ğ“¸) â†’` Term is a (Ï ğ“¸)-tuple of terms, each with interpretation :math:`(ğŸ i)^ğš¨`, then we take :math:`t^ğ€(ğŸ)` to be :math:`ğ“¸^ğ€ \bigl( Î» \{ (i : Ï ğ“¸) . (ğŸ i)^ğ€\}\bigr)`.

-- Let's translate this definition using the Agda syntax we developed above.

-- Let ``t`` be a term, ğ€ an algebra,  of signature ``S``.

-- The **interpretation** of :math:`t` in ğ€---often denoted in the literature by :math:`t^ğš¨`---is an operation of :math:`A` defined by recursion on the structure of :math:`t`.

-- 1. If ``t`` is a variable, say, ``x : X``, then we define ``(t Ì‚ A) : âŸ¦ A âŸ§áµ¤ -> âŸ¦ A âŸ§áµ¤`` for each ``a : âŸ¦ A âŸ§áµ¤`` by ``(t Ì‚ A) a = a``.
-- 2. If ``t = ğ“¸ ğŸ``, where ``ğ“¸ : âŸ¨ S âŸ©â‚’`` is a basic operation symbol with interpretation ``A âŸ¦ ğ“¸ âŸ§`` in ğš¨, and if ``ğŸ : âŸ¨ S âŸ©â‚ ğ“¸ -> Term`` is a ``(âŸ¨ S âŸ©â‚ ğ“¸)``-tuple of terms with interpretations ``(ğŸ i) Ì‚ A`` for each ``i : âŸ¨ S âŸ©â‚ ğ“¸``, then we define
--    ``(t Ì‚ A) = (ğ“¸ ğŸ) Ì‚ A = (A âŸ¦ ğ“¸ âŸ§) Î»{i -> (ğŸ i) Ì‚ A}``

-- Here's how we would implement this in Agda.
-- .. code-block:: agda
--    _Ì‚_ : {â„“â‚ : Level} -> Term -> (A : algebra {â„“â‚} S) -> (X -> âŸ¦ A âŸ§áµ¤) -> âŸ¦ A âŸ§áµ¤
--    ((generator x) Ì‚ A) tup = tup x
--    ((node ğ“¸ args) Ì‚ A) tup = (A âŸ¦ ğ“¸ âŸ§) Î»{i -> (args i Ì‚ A) tup }


-- open import Level
-- open import Agda.Builtin.Nat public
--   renaming ( Nat to â„•; _-_ to _âˆ¸_; zero to nzero; suc to succ )
-- open import Data.Product using (Î£; _,_; âˆƒ; Î£-syntax; âˆƒ-syntax; _Ã—_)
-- open import Relation.Unary hiding (_âŠ†_;_â‡’_)
-- -- open import Relation.Binary.Core using (IsEquivalence)
-- --open import Relation.Binary using (IsEquivalence)
-- import Relation.Binary.PropositionalEquality as Eq
--   hiding (setoid; Reveal_Â·_is_;[_];âˆ€-extensionality)
-- open Eq using (_â‰¡_; refl; cong; sym)
-- open Eq.â‰¡-Reasoning
-- open import Function using (_âˆ˜_)
-- open import Function.Equality renaming (_âˆ˜_ to _âˆ˜â‚›_) hiding (cong)

-- open import Relation.Nullary using (Â¬_)
-- open import Relation.Nullary.Negation using ()
--   renaming (contradiction to Â¬Â¬-intro)
--  using    ( _+_; _*_ )

-- open import Data.Fin public
--   -- (See "NOTE on Fin" section below)
--   hiding ( _+_; _<_ )
--   renaming ( suc to fsucc; zero to fzero )
--------------------------------------------------------------
-- open import preliminaries  using (_âŠ_ ; âˆ€-extensionality; âˆ‘; List)
