
{-# OPTIONS --without-K --exact-split --safe #-}

open import Overture using (𝓞 ; 𝓥 ; Signature)

module Setoid.Homomorphisms.Isomorphisms {𝑆 : Signature 𝓞 𝓥}  where

open import Agda.Primitive              using ()      renaming ( Set to Type )
open import Data.Product                using ( _,_ )
open import Data.Unit.Polymorphic.Base  using ()      renaming ( ⊤ to 𝟙 ; tt to ∗ )
open import Data.Unit.Base              using ( ⊤ ; tt )
open import Function                    using ( id )  renaming ( Func to _⟶_ )
open import Level                       using ( Level ; Lift ; lift ; lower ; _⊔_ )
open import Relation.Binary             using ( Setoid ; Reflexive ; Sym ; Trans )

open import Relation.Binary.PropositionalEquality as ≡ using ()

open import Overture          using ( ∣_∣ ; ∥_∥ )
open import Setoid.Functions  using ( _⊙_ ; eq ; IsInjective ; IsSurjective )

open import Setoid.Algebras {𝑆 = 𝑆}  using ( Algebra ; Lift-Alg ; _̂_ )
                                     using ( Lift-Algˡ ; Lift-Algʳ ; ⨅ )

open import Setoid.Homomorphisms.Basic       {𝑆 = 𝑆} using  ( hom ; IsHom )
open import Setoid.Homomorphisms.Properties  {𝑆 = 𝑆} using
 ( 𝒾𝒹 ; ⊙-hom ; ToLiftˡ ; FromLiftˡ ; ToFromLiftˡ ; FromToLiftˡ
 ; ToLiftʳ ; FromLiftʳ ; ToFromLiftʳ ; FromToLiftʳ )

open _⟶_      using ( cong ) renaming ( to to _⟨$⟩_ )
open Algebra  using ( Domain )

private variable  α ρᵃ β ρᵇ γ ρᶜ ι : Level

module _ (𝑨 : Algebra α ρᵃ) (𝑩 : Algebra β ρᵇ) where
 open Setoid (Domain 𝑨) using ( sym ; trans ) renaming ( _≈_ to _≈₁_ )
 open Setoid (Domain 𝑩) using () renaming ( _≈_ to _≈₂_ ; sym to sym₂ ; trans to trans₂)

 record _≅_ : Type (𝓞 ⊔ 𝓥 ⊔ α ⊔ β ⊔ ρᵃ ⊔ ρᵇ ) where
  constructor mkiso
  field
   to : hom 𝑨 𝑩
   from : hom 𝑩 𝑨
   to∼from : ∀ b → (∣ to ∣ ⟨$⟩ (∣ from ∣ ⟨$⟩ b)) ≈₂ b
   from∼to : ∀ a → (∣ from ∣ ⟨$⟩ (∣ to ∣ ⟨$⟩ a)) ≈₁ a

  toIsSurjective : IsSurjective ∣ to ∣
  toIsSurjective {y} = eq (∣ from ∣ ⟨$⟩ y) (sym₂ (to∼from y))

  toIsInjective : IsInjective ∣ to ∣
  toIsInjective {x} {y} xy = Goal
   where
   ξ : ∣ from ∣ ⟨$⟩ (∣ to ∣ ⟨$⟩ x) ≈₁ ∣ from ∣ ⟨$⟩ (∣ to ∣ ⟨$⟩ y)
   ξ = cong ∣ from ∣ xy
   Goal : x ≈₁ y
   Goal = trans (sym (from∼to x)) (trans ξ (from∼to y))

  fromIsSurjective : IsSurjective ∣ from ∣
  fromIsSurjective {y} = eq (∣ to ∣ ⟨$⟩ y) (sym (from∼to y))

  fromIsInjective : IsInjective ∣ from ∣
  fromIsInjective {x} {y} xy = Goal
   where
   ξ : ∣ to ∣ ⟨$⟩ (∣ from ∣ ⟨$⟩ x) ≈₂ ∣ to ∣ ⟨$⟩ (∣ from ∣ ⟨$⟩ y)
   ξ = cong ∣ to ∣ xy
   Goal : x ≈₂ y
   Goal = trans₂ (sym₂ (to∼from x)) (trans₂ ξ (to∼from y))

open _≅_

≅-refl : Reflexive (_≅_ {α}{ρᵃ})
≅-refl {α}{ρᵃ}{𝑨} = mkiso 𝒾𝒹 𝒾𝒹 (λ b → refl) λ a → refl
 where open Setoid (Domain 𝑨) using ( refl )

≅-sym : Sym (_≅_{β}{ρᵇ}) (_≅_{α}{ρᵃ})
≅-sym φ = mkiso (from φ) (to φ) (from∼to φ) (to∼from φ)

≅-trans : Trans (_≅_ {α}{ρᵃ})(_≅_{β}{ρᵇ})(_≅_{α}{ρᵃ}{γ}{ρᶜ})
≅-trans {ρᶜ = ρᶜ}{𝑨}{𝑩}{𝑪} ab bc = mkiso f g τ ν
  where
  open Setoid (Domain 𝑨) using () renaming ( _≈_ to _≈₁_ ; trans to trans₁ )
  open Setoid (Domain 𝑪) using () renaming ( _≈_ to _≈₃_ ; trans to trans₃ )
  f : hom 𝑨 𝑪
  f = ⊙-hom (to ab) (to bc)

  g : hom 𝑪 𝑨
  g = ⊙-hom (from bc) (from ab)

  τ : ∀ b → (∣ f ∣ ⟨$⟩ (∣ g ∣ ⟨$⟩ b)) ≈₃ b
  τ b = trans₃ (cong ∣ to bc ∣ (to∼from ab (∣ from bc ∣ ⟨$⟩ b))) (to∼from bc b)

  ν : ∀ a → (∣ g ∣ ⟨$⟩ (∣ f ∣ ⟨$⟩ a)) ≈₁ a
  ν a = trans₁ (cong ∣ from ab ∣ (from∼to bc (∣ to ab ∣ ⟨$⟩ a))) (from∼to ab a)

module _ {𝑨 : Algebra α ρᵃ}{𝑩 : Algebra β ρᵇ} where
 open Setoid (Domain 𝑨) using ( _≈_ ; sym ; trans )

 ≅toInjective : (φ : 𝑨 ≅ 𝑩) → IsInjective ∣ to φ ∣
 ≅toInjective (mkiso (f , _) (g , _) _ g∼f){a₀}{a₁} fafb = Goal
  where
  lem1 : a₀ ≈ (g ⟨$⟩ (f ⟨$⟩ a₀))
  lem1 = sym (g∼f a₀)
  lem2 : (g ⟨$⟩ (f ⟨$⟩ a₀)) ≈ (g ⟨$⟩ (f ⟨$⟩ a₁))
  lem2 = cong g fafb
  lem3 : (g ⟨$⟩ (f ⟨$⟩ a₁)) ≈ a₁
  lem3 = g∼f a₁
  Goal : a₀ ≈ a₁
  Goal = trans lem1 (trans lem2 lem3)

≅fromInjective :  {𝑨 : Algebra α ρᵃ}{𝑩 : Algebra β ρᵇ}
                  (φ : 𝑨 ≅ 𝑩) → IsInjective ∣ from φ ∣

≅fromInjective φ = ≅toInjective (≅-sym φ)

module _ {𝑨 : Algebra α ρᵃ}{ℓ : Level} where
 Lift-≅ˡ : 𝑨 ≅ (Lift-Algˡ 𝑨 ℓ)
 Lift-≅ˡ = mkiso ToLiftˡ FromLiftˡ (ToFromLiftˡ{𝑨 = 𝑨}) (FromToLiftˡ{𝑨 = 𝑨}{ℓ})

 Lift-≅ʳ : 𝑨 ≅ (Lift-Algʳ 𝑨 ℓ)
 Lift-≅ʳ = mkiso ToLiftʳ FromLiftʳ (ToFromLiftʳ{𝑨 = 𝑨}) (FromToLiftʳ{𝑨 = 𝑨}{ℓ})

Lift-≅ : {𝑨 : Algebra α ρᵃ}{ℓ ρ : Level} → 𝑨 ≅ (Lift-Alg 𝑨 ℓ ρ)
Lift-≅ = ≅-trans Lift-≅ˡ Lift-≅ʳ

module _ {𝑨 : Algebra α ρᵃ}{𝑩 : Algebra β ρᵇ}{ℓᵃ ℓᵇ : Level} where

 Lift-Alg-isoˡ : 𝑨 ≅ 𝑩 → Lift-Algˡ 𝑨 ℓᵃ ≅ Lift-Algˡ 𝑩 ℓᵇ
 Lift-Alg-isoˡ A≅B = ≅-trans (≅-trans (≅-sym Lift-≅ˡ ) A≅B) Lift-≅ˡ

 Lift-Alg-isoʳ : 𝑨 ≅ 𝑩 →  Lift-Algʳ 𝑨 ℓᵃ ≅ Lift-Algʳ 𝑩 ℓᵇ
 Lift-Alg-isoʳ A≅B = ≅-trans (≅-trans (≅-sym Lift-≅ʳ ) A≅B) Lift-≅ʳ

Lift-Alg-iso :  {𝑨 : Algebra α ρᵃ}{𝑩 : Algebra β ρᵇ}{ℓᵃ rᵃ ℓᵇ rᵇ : Level}
 →              𝑨 ≅ 𝑩 → Lift-Alg 𝑨 ℓᵃ rᵃ ≅ Lift-Alg 𝑩 ℓᵇ rᵇ
Lift-Alg-iso {ℓᵇ = ℓᵇ} A≅B =
  ≅-trans  (Lift-Alg-isoʳ{ℓᵇ = ℓᵇ}(≅-trans (Lift-Alg-isoˡ{ℓᵇ = ℓᵇ} A≅B) (≅-sym Lift-≅ˡ)))
           (Lift-Alg-isoʳ Lift-≅ˡ)

module _ {𝑨 : Algebra α ρᵃ}{ℓ₁ ℓ₂ : Level} where

 Lift-assocˡ : Lift-Algˡ 𝑨 (ℓ₁ ⊔ ℓ₂) ≅  Lift-Algˡ (Lift-Algˡ 𝑨 ℓ₁) ℓ₂
 Lift-assocˡ = ≅-trans (≅-trans (≅-sym Lift-≅ˡ) Lift-≅ˡ) Lift-≅ˡ

 Lift-assocʳ : Lift-Algʳ 𝑨 (ℓ₁ ⊔ ℓ₂) ≅  Lift-Algʳ (Lift-Algʳ 𝑨 ℓ₁) ℓ₂
 Lift-assocʳ = ≅-trans (≅-trans (≅-sym Lift-≅ʳ) Lift-≅ʳ) Lift-≅ʳ

Lift-assoc :  {𝑨 : Algebra α ρᵃ}{ℓ ρ : Level}
 →            Lift-Alg 𝑨 ℓ ρ ≅  Lift-Algʳ (Lift-Algˡ 𝑨 ℓ) ρ
Lift-assoc {𝑨 = 𝑨}{ℓ}{ρ} = ≅-trans (≅-sym Lift-≅) (≅-trans Lift-≅ˡ Lift-≅ʳ)

Lift-assoc' :  {𝑨 : Algebra α α}{β γ : Level}
 →             Lift-Alg 𝑨 (β ⊔ γ) (β ⊔ γ) ≅ Lift-Alg (Lift-Alg 𝑨 β β) γ γ
Lift-assoc'{𝑨 = 𝑨}{β}{γ} = ≅-trans (≅-sym Lift-≅) (≅-trans Lift-≅ Lift-≅)

module _ {𝓘 : Level}{I : Type 𝓘} {𝒜 : I → Algebra α ρᵃ} {ℬ : I → Algebra β ρᵇ} where
 open Algebra (⨅ 𝒜)  using () renaming (Domain to ⨅A )
 open Setoid ⨅A      using () renaming ( _≈_ to _≈₁_ )
 open Algebra (⨅ ℬ)  using () renaming (Domain to ⨅B )
 open Setoid ⨅B      using () renaming ( _≈_ to _≈₂_ )
 open IsHom

 ⨅≅ : (∀ (i : I) → 𝒜 i ≅ ℬ i) → ⨅ 𝒜 ≅ ⨅ ℬ
 ⨅≅ AB = mkiso (ϕ , ϕhom) (ψ , ψhom) ϕ∼ψ ψ∼ϕ
  where
   ϕ : ⨅A ⟶ ⨅B
   ϕ = record  { to = λ a i → ∣ to (AB i) ∣ ⟨$⟩ (a i)
               ; cong = λ a i → cong ∣ to (AB i) ∣ (a i)
               }

   ϕhom : IsHom (⨅ 𝒜) (⨅ ℬ) ϕ
   ϕhom = record { compatible = λ i → compatible ∥ to (AB i) ∥ }

   ψ : ⨅B ⟶ ⨅A
   ψ = record  { to = λ b i → ∣ from (AB i) ∣ ⟨$⟩ (b i)
               ; cong = λ b i → cong ∣ from (AB i) ∣ (b i)
               }

   ψhom : IsHom (⨅ ℬ) (⨅ 𝒜) ψ
   ψhom = record { compatible = λ i → compatible ∥ from (AB i) ∥ }

   ϕ∼ψ : ∀ b → (ϕ ⟨$⟩ (ψ ⟨$⟩ b)) ≈₂ b
   ϕ∼ψ b = λ i → to∼from (AB i) (b i)

   ψ∼ϕ : ∀ a → (ψ ⟨$⟩ (ϕ ⟨$⟩ a)) ≈₁ a
   ψ∼ϕ a = λ i → from∼to (AB i)(a i)

module _  {𝓘 : Level}{I : Type 𝓘}
          {𝒜 : I → Algebra α ρᵃ}
          {ℬ : (Lift γ I) → Algebra β ρᵇ} where

 open Algebra (⨅ 𝒜)  using () renaming (Domain to ⨅A )
 open Setoid ⨅A      using () renaming ( _≈_ to _≈₁_ )
 open Algebra (⨅ ℬ)  using () renaming (Domain to ⨅B )
 open Setoid ⨅B      using () renaming ( _≈_ to _≈₂_ )
 open IsHom

 Lift-Alg-⨅≅ˡ : (∀ i → 𝒜 i ≅ ℬ (lift i)) → Lift-Algˡ (⨅ 𝒜) γ ≅ ⨅ ℬ
 Lift-Alg-⨅≅ˡ AB = ≅-trans (≅-sym Lift-≅ˡ) A≅B
  where
   ϕ : ⨅A ⟶ ⨅B
   ϕ = record  { to = λ a i → ∣ to (AB (lower i)) ∣ ⟨$⟩ (a (lower i))
               ; cong = λ a i → cong ∣ to (AB (lower i)) ∣ (a (lower i))
               }

   ϕhom : IsHom (⨅ 𝒜) (⨅ ℬ) ϕ
   ϕhom = record { compatible = λ i → compatible ∥ to (AB (lower i)) ∥ }

   ψ : ⨅B ⟶ ⨅A
   ψ = record  { to = λ b i → ∣ from (AB i) ∣ ⟨$⟩ (b (lift i))
               ; cong = λ b i → cong ∣ from (AB i) ∣ (b (lift i))
               }

   ψhom : IsHom (⨅ ℬ) (⨅ 𝒜) ψ
   ψhom = record { compatible = λ i → compatible ∥ from (AB i) ∥ }

   ϕ∼ψ : ∀ b → (ϕ ⟨$⟩ (ψ ⟨$⟩ b)) ≈₂ b
   ϕ∼ψ b = λ i → to∼from (AB (lower i)) (b i)

   ψ∼ϕ : ∀ a → (ψ ⟨$⟩ (ϕ ⟨$⟩ a)) ≈₁ a
   ψ∼ϕ a = λ i → from∼to (AB i)(a i)

   A≅B : ⨅ 𝒜 ≅ ⨅ ℬ
   A≅B = mkiso (ϕ , ϕhom) (ψ , ψhom) ϕ∼ψ ψ∼ϕ

module _ {𝓘 : Level}{I : Type 𝓘} {𝒜 : I → Algebra α ρᵃ} where
 open IsHom
 open Algebra  using (Domain)
 open Setoid   using (_≈_ )

 ⨅≅⨅ℓ : ∀ {ℓ} → ⨅ 𝒜 ≅ ⨅ (λ i → Lift-Alg (𝒜 (lower{ℓ = ℓ} i)) ℓ ℓ)
 ⨅≅⨅ℓ {ℓ} = mkiso (φ , φhom) (ψ , ψhom) φ∼ψ ψ∼φ
  where
  open Algebra (⨅ 𝒜)  using () renaming (Domain to ⨅A )
  open Setoid ⨅A      using () renaming ( _≈_ to _≈₁_ )

  ⨅ℓ𝒜 : Algebra _ _
  ⨅ℓ𝒜 = ⨅ (λ i → Lift-Alg (𝒜 (lower{ℓ = ℓ} i)) ℓ ℓ)

  open Algebra ⨅ℓ𝒜 using () renaming (Domain to ⨅ℓA)

  φ : ⨅A ⟶ ⨅ℓA
  (φ ⟨$⟩ x) i = lift (x (lower i))
  cong φ x i = lift (x (lower i))
  φhom : IsHom (⨅ 𝒜) ⨅ℓ𝒜  φ
  compatible φhom i = lift refl
   where open Setoid (Domain (𝒜 (lower i))) using ( refl )

  ψ : ⨅ℓA ⟶ ⨅A
  (ψ ⟨$⟩ x) i = lower (x (lift i))
  cong ψ x i = lower (x (lift i))
  ψhom : IsHom ⨅ℓ𝒜 (⨅ 𝒜) ψ
  compatible ψhom i = refl
   where open Setoid (Domain (𝒜 i)) using ( refl )

  φ∼ψ : ∀ b i → (Domain (Lift-Alg (𝒜 (lower i)) ℓ ℓ)) ._≈_ ((φ ⟨$⟩ (ψ ⟨$⟩ b)) i) (b i)
  φ∼ψ _ i = lift (reflexive ≡.refl)
   where open Setoid (Domain (𝒜 (lower i))) using ( reflexive )

  ψ∼φ : ∀ a i → (Domain (𝒜 i)) ._≈_ ((ψ ⟨$⟩ (φ ⟨$⟩ a)) i) (a i)
  ψ∼φ _ i = (reflexive ≡.refl)
   where open Setoid (Domain (𝒜  i)) using ( reflexive )

module _ {ι : Level}{I : Type ι}{𝒜 : I → Algebra α ρᵃ} where
 open IsHom
 open Algebra  using (Domain)
 open Setoid   using (_≈_ )

 ⨅≅⨅ℓρ : ∀ {ℓ ρ} → ⨅ 𝒜 ≅ ⨅ (λ i → Lift-Alg (𝒜 i) ℓ ρ)
 ⨅≅⨅ℓρ {ℓ}{ρ} = mkiso φ ψ φ∼ψ ψ∼φ
  where
  open Algebra (⨅ 𝒜)                         using () renaming ( Domain to ⨅A )
  open Setoid ⨅A                             using () renaming ( _≈_ to _≈⨅A≈_ )
  open Algebra (⨅ λ i → Lift-Alg (𝒜 i) ℓ ρ)  using () renaming ( Domain to ⨅lA )
  open Setoid ⨅lA                            using () renaming ( _≈_ to _≈⨅lA≈_ )

  φfunc : ⨅A ⟶ ⨅lA
  (φfunc ⟨$⟩ x) i = lift (x i)
  cong φfunc x i = lift (x i)

  φhom : IsHom (⨅ 𝒜) (⨅ λ i → Lift-Alg (𝒜 i) ℓ ρ) φfunc
  compatible φhom i = refl
   where open Setoid (Domain (Lift-Alg (𝒜 i) ℓ ρ)) using ( refl )

  φ : hom (⨅ 𝒜) (⨅ λ i → Lift-Alg (𝒜 i) ℓ ρ)
  φ = φfunc , φhom

  ψfunc : ⨅lA ⟶ ⨅A
  (ψfunc ⟨$⟩ x) i = lower (x i)
  cong ψfunc x i = lower (x i)

  ψhom : IsHom (⨅ λ i → Lift-Alg (𝒜 i) ℓ ρ) (⨅ 𝒜) ψfunc
  compatible ψhom i = refl
   where open Setoid (Domain (𝒜 i)) using (refl)

  ψ : hom (⨅ λ i → Lift-Alg (𝒜 i) ℓ ρ) (⨅ 𝒜)
  ψ = ψfunc , ψhom

  φ∼ψ : ∀ b → ∣ φ ∣ ⟨$⟩ (∣ ψ ∣ ⟨$⟩ b) ≈⨅lA≈ b
  φ∼ψ _ i = reflexive ≡.refl
   where open Setoid (Domain (Lift-Alg (𝒜 i) ℓ ρ)) using ( reflexive )

  ψ∼φ : ∀ a → ∣ ψ ∣ ⟨$⟩ (∣ φ ∣ ⟨$⟩ a) ≈⨅A≈ a
  ψ∼φ _ = reflexive ≡.refl
   where open Setoid (Domain (⨅ 𝒜)) using ( reflexive )

module _ {ℓᵃ : Level}{I : Type ℓᵃ}{𝒜 : I → Algebra α ρᵃ}where
 open IsHom
 open Algebra  using (Domain)
 open Setoid   using (_≈_ )

 ⨅≅⨅lowerℓρ : ∀ {ℓ ρ} → ⨅ 𝒜 ≅ ⨅ λ i → Lift-Alg (𝒜 (lower{ℓ = α ⊔ ρᵃ} i)) ℓ ρ
 ⨅≅⨅lowerℓρ {ℓ}{ρ} = mkiso φ ψ φ∼ψ ψ∼φ
  where
  open Algebra (⨅ 𝒜)                               using() renaming ( Domain to ⨅A )
  open Setoid ⨅A                                   using() renaming ( _≈_ to _≈⨅A≈_ )
  open Algebra(⨅ λ i → Lift-Alg(𝒜 (lower i)) ℓ ρ)  using() renaming ( Domain to ⨅lA )
  open Setoid ⨅lA                                  using() renaming ( _≈_ to _≈⨅lA≈_ )

  φfunc : ⨅A ⟶ ⨅lA
  (φfunc ⟨$⟩ x) i = lift (x (lower i))
  cong φfunc x i = lift (x (lower i))

  φhom : IsHom (⨅ 𝒜) (⨅ λ i → Lift-Alg (𝒜 (lower i)) ℓ ρ) φfunc
  compatible φhom i = refl
   where open Setoid (Domain (Lift-Alg (𝒜 (lower i)) ℓ ρ)) using ( refl )

  φ : hom (⨅ 𝒜) (⨅ λ i → Lift-Alg (𝒜 (lower i)) ℓ ρ)
  φ = φfunc , φhom

  ψfunc : ⨅lA ⟶ ⨅A
  (ψfunc ⟨$⟩ x) i = lower (x (lift i))
  cong ψfunc x i = lower (x (lift i))

  ψhom : IsHom (⨅ λ i → Lift-Alg (𝒜 (lower i)) ℓ ρ) (⨅ 𝒜) ψfunc
  compatible ψhom i = refl
   where open Setoid (Domain (𝒜 i)) using (refl)

  ψ : hom (⨅ λ i → Lift-Alg (𝒜 (lower i)) ℓ ρ) (⨅ 𝒜)
  ψ = ψfunc , ψhom

  φ∼ψ : ∀ b → ∣ φ ∣ ⟨$⟩ (∣ ψ ∣ ⟨$⟩ b) ≈⨅lA≈ b
  φ∼ψ _ i = reflexive ≡.refl
   where open Setoid (Domain (Lift-Alg (𝒜 (lower i)) ℓ ρ)) using (reflexive)

  ψ∼φ : ∀ a → ∣ ψ ∣ ⟨$⟩ (∣ φ ∣ ⟨$⟩ a) ≈⨅A≈ a
  ψ∼φ _ = reflexive ≡.refl
   where open Setoid (Domain (⨅ 𝒜)) using (reflexive)

 ℓ⨅≅⨅ℓ : ∀ {ℓ} → Lift-Alg (⨅ 𝒜) ℓ ℓ ≅ ⨅ λ i → Lift-Alg (𝒜 (lower{ℓ = ℓ} i)) ℓ ℓ
 ℓ⨅≅⨅ℓ {ℓ} = mkiso (φ , φhom) (ψ , ψhom) φ∼ψ ψ∼φ -- φ∼ψ ψ∼φ
  where
  ℓ⨅𝒜 : Algebra _ _
  ℓ⨅𝒜 = Lift-Alg (⨅ 𝒜) ℓ ℓ
  ⨅ℓ𝒜 : Algebra _ _
  ⨅ℓ𝒜 = ⨅ (λ i → Lift-Alg (𝒜 (lower{ℓ = ℓ} i)) ℓ ℓ)

  open Algebra ℓ⨅𝒜  using() renaming (Domain to ℓ⨅A )
  open Setoid ℓ⨅A   using() renaming ( _≈_ to _≈₁_ )
  open Algebra ⨅ℓ𝒜  using() renaming (Domain to ⨅ℓA)
  open Setoid ⨅ℓA   using() renaming ( _≈_ to _≈₂_ )

  φ : ℓ⨅A ⟶ ⨅ℓA
  (φ ⟨$⟩ x) i = lift ((lower x)(lower i))
  cong φ x i = lift ((lower x)(lower i))
  φhom : IsHom ℓ⨅𝒜 ⨅ℓ𝒜  φ
  compatible φhom i = lift refl
   where open Setoid (Domain (𝒜 (lower i))) using ( refl )

  ψ : ⨅ℓA ⟶ ℓ⨅A
  (ψ ⟨$⟩ x) = lift λ i → lower (x (lift i))
  cong ψ x = lift λ i → lower (x (lift i))
  ψhom : IsHom ⨅ℓ𝒜 ℓ⨅𝒜 ψ
  lower (compatible ψhom) i = refl
   where open Setoid (Domain (𝒜 i)) using ( refl )

  φ∼ψ : ∀ b → (φ ⟨$⟩ (ψ ⟨$⟩ b)) ≈₂ b
  lower (φ∼ψ _ i) = reflexive ≡.refl
   where open Setoid (Domain (𝒜 (lower i))) using ( reflexive )

  ψ∼φ : ∀ a → (ψ ⟨$⟩ (φ ⟨$⟩ a)) ≈₁ a
  lower (ψ∼φ _) i = reflexive ≡.refl
   where open Setoid (Domain (𝒜  i)) using ( reflexive )

module _ {ι : Level}{𝑨 : Algebra α ρᵃ} where
 open Algebra 𝑨                     using() renaming ( Domain to A )
 open Algebra (⨅ λ (i : 𝟙{ι}) → 𝑨)  using() renaming ( Domain to ⨅A )
 open Setoid A                      using ( refl )
 open _≅_
 open IsHom

 private
  to𝟙 : A ⟶ ⨅A
  (to𝟙 ⟨$⟩ x) ∗ = x
  cong to𝟙 xy ∗ = xy
  from𝟙 : ⨅A ⟶ A
  from𝟙 ⟨$⟩ x = x ∗
  cong from𝟙 xy = xy ∗

  to𝟙IsHom : IsHom 𝑨 (⨅ (λ _ → 𝑨)) to𝟙
  compatible to𝟙IsHom = λ _ → refl
  from𝟙IsHom : IsHom (⨅ (λ _ → 𝑨)) 𝑨 from𝟙
  compatible from𝟙IsHom = refl

 ≅⨅⁺-refl : 𝑨 ≅ ⨅ (λ (i : 𝟙) → 𝑨)
 to ≅⨅⁺-refl = to𝟙 , to𝟙IsHom
 from ≅⨅⁺-refl = from𝟙 , from𝟙IsHom
 to∼from ≅⨅⁺-refl = λ _ _ → refl
 from∼to ≅⨅⁺-refl = λ _ → refl

module _ {𝑨 : Algebra α ρᵃ} where
 open Algebra 𝑨                  using () renaming ( Domain to A )
 open Algebra (⨅ λ (i : ⊤) → 𝑨)  using () renaming ( Domain to ⨅A )
 open Setoid A                   using ( refl )
 open _≅_
 open IsHom

 private
  to⊤ : A ⟶ ⨅A
  (to⊤ ⟨$⟩ x) = λ _ → x
  cong to⊤ xy = λ _ → xy
  from⊤ : ⨅A ⟶ A
  from⊤ ⟨$⟩ x = x tt
  cong from⊤ xy = xy tt

  to⊤IsHom : IsHom 𝑨 (⨅ λ _ → 𝑨) to⊤
  compatible to⊤IsHom = λ _ → refl
  from⊤IsHom : IsHom (⨅ λ _ → 𝑨) 𝑨 from⊤
  compatible from⊤IsHom = refl

 ≅⨅-refl : 𝑨 ≅ ⨅ (λ (i : ⊤) → 𝑨)
 to ≅⨅-refl = to⊤ , to⊤IsHom
 from ≅⨅-refl = from⊤ , from⊤IsHom
 to∼from ≅⨅-refl = λ _ _ → refl
 from∼to ≅⨅-refl = λ _ → refl

